Implement initial version of rm_chain. Partially prove derivers => rm_chain

Escallon/LR_Parsing/LR_Parser.thy
@@ -123,7 +123,7 @@ lemma step_is_eps_stepn:
   using assms by cases auto
 
 
-lemma steps_impl_eps_stepn:
+lemma steps_imp_eps_stepn:
   assumes "c0 \<turnstile>* c1"
   obtains n where "c0 \<turnstile>\<epsilon>(n) c1"
   using assms proof (induction arbitrary: thesis)
@@ -138,7 +138,7 @@ next
      (metis step(2,3,4) nfa.eps_stepn.eps nfa_axioms old.prod.exhaust))
 qed
 
-lemma eps_stepn_impl_steps: "c0 \<turnstile>\<epsilon>(n) c1 \<Longrightarrow> c0 \<turnstile>* c1" 
+lemma eps_stepn_imp_steps: "c0 \<turnstile>\<epsilon>(n) c1 \<Longrightarrow> c0 \<turnstile>* c1" 
   by (induction rule: eps_stepn.induct) auto
 
 (* To be used in proof of Theorem 3.4.1 *)
@@ -150,7 +150,7 @@ lemma last_eps_step:
   from less(3) show ?case 
   proof cases
     case (nxt q a)
-    with steps_len_dec eps_stepn_impl_steps have  "length u \<ge> length (a#w)" by blast
+    with steps_len_dec eps_stepn_imp_steps have  "length u \<ge> length (a#w)" by blast
     then have "length u - length (a#w) < length u - length w" by auto
     then show ?thesis using less nxt by blast
   qed (use less in blast)
@@ -241,8 +241,8 @@ abbreviation IPDA_stepn :: "('n,'t) item list \<times> 't list \<Rightarrow> nat
 
 
 
-
 (*
+
 lemma char_init_step_is_eps:
   assumes "([S' \<rightarrow> [] . [Nt S]], \<gamma>) \<turnstile>c ([A \<rightarrow> \<alpha> . \<beta>], \<gamma>')" (is "(?S,_) \<turnstile>c _")
   shows "A = S \<and> \<gamma> = \<gamma>'"
@@ -272,7 +272,7 @@ lemma char_init_noeps_eq:
         using S'_def S_def less.prems(3) sorry
     next
       case (nxt p a)
-      from char_fa.eps_stepn_impl_steps[OF nxt(1)] char_fa.steps_len_dec have "length (a#u) \<le> length \<gamma>"
+      from char_fa.eps_stepn_imp_steps[OF nxt(1)] char_fa.steps_len_dec have "length (a#u) \<le> length \<gamma>"
         by presburger
       hence "length \<gamma> - length (a#u) < length \<gamma> - length u" by simp
       then show ?thesis 
@@ -282,12 +282,12 @@ lemma char_init_noeps_eq:
   qed
 qed presburger
 
-lemma char_fa_comp_impl_deriver:
+lemma char_fa_comp_imp_deriver:
     assumes "([S' \<rightarrow> [] . [Nt S]], \<gamma>) \<turnstile>c* ([A \<rightarrow> \<alpha> . \<beta>], [])"
     obtains w \<gamma>' where "Prods G' \<turnstile> [Nt S'] \<Rightarrow>r* \<gamma>'@Nt A#w" "Prods G' \<turnstile> \<gamma>'@Nt A#w \<Rightarrow>r \<gamma>'@\<alpha>@\<beta>@w" "\<gamma> = \<gamma>'@\<alpha>"
 proof -
   from assms obtain n where "([S' \<rightarrow> [] . [Nt S]], \<gamma>) \<turnstile>\<epsilon>(n) ([A \<rightarrow> \<alpha> . \<beta>], [])"
-    using char_fa.steps_impl_eps_stepn by blast
+    using char_fa.steps_imp_eps_stepn by blast
   with that show ?thesis
   proof (induction n arbitrary: A \<alpha> \<beta>)
     case 0
@@ -329,11 +329,11 @@ lemma deriver_decomp_reachable:
   shows "P \<turnstile> A \<Rightarrow>r* take i (concat \<alpha>) @ Nt (X!i) # rev (take i (map Tm (concat v)))"
   sorry 
 
-*)
 
 
 
-lemma eq_tl_impl_substring:
+
+lemma eq_tl_imp_substring:
   assumes "length u \<ge> length v"
   "xs @ u = ys @ v"
 obtains w where "w @ v = u"
@@ -349,10 +349,10 @@ lemma deriver_decomp:
   oops
 (*proof -
   obtain xs where xs_def: "\<gamma> @ Nt A # map Tm w = \<alpha> @ xs @ map Tm u" "(X, xs) \<in> P" 
-    using deriver_impl_in_Prods[OF assms] by metis
+    using deriver_imp_in_Prods[OF assms] by metis
   moreover have "length w \<ge> length u" using assms sorry
   ultimately obtain zs :: "('a,'b) syms" where zs_def: "zs @ map Tm u = map Tm w" 
-    using eq_tl_impl_substring[of "map Tm u" "map Tm w"] 
+    using eq_tl_imp_substring[of "map Tm u" "map Tm w"] 
     by (metis append.assoc append_Cons append_Nil length_map)
   then obtain ys where "xs = ys@zs" "\<delta>@ys = \<gamma>'@[Nt A]"
   proof -
@@ -371,7 +371,7 @@ definition toitems :: "'n list \<Rightarrow> ('n,'t) syms list \<Rightarrow> ('n
     map2 (\<lambda>(Xi, Xsi) (\<alpha>si,\<beta>si). [Xi \<rightarrow> \<alpha>si . Nt Xsi # \<beta>si]) Xs \<alpha>\<beta>)"
 
 
-lemma derivers_S_append_impl_comp:
+lemma derivers_S_append_imp_comp:
   assumes "Prods G' \<turnstile> \<beta> \<Rightarrow>r* map Tm w"
     "\<alpha>@\<beta> = [Nt S]"
   shows "([[S' \<rightarrow> \<alpha> . \<beta>], init_symbol IPDA], w) \<turnstile>P* ([I.final_state, init_symbol IPDA], [])"
@@ -381,14 +381,14 @@ proof -
   then show ?thesis
   proof cases
     case init
-    with assms(1) have "w \<in> LangS G'" using G'_derives_from_S_impl_in_Lang
+    with assms(1) have "w \<in> LangS G'" using G'_derives_from_S_imp_in_Lang
       by (simp add: derivers_imp_derives)
     then show ?thesis using I.Lang_eq_Lang_G Lang_preserved I.init_state_ipda init 
       unfolding I.Lang_def by auto
   qed (use assms(1) derivers_imp_derives in force)
 qed
 
-lemma derivers_impl_in_stack:
+lemma derivers_imp_in_stack:
   assumes "Prods G' \<turnstile> [Nt S'] \<Rightarrow>r* \<gamma>@Nt A#map Tm w"
     "Prods G' \<turnstile> \<gamma>@Nt A#map Tm w \<Rightarrow>r \<gamma>@\<alpha>@map Tm w"
     "\<gamma>@\<alpha>@map Tm w = \<delta>@Nt B#map Tm u"
@@ -402,7 +402,7 @@ lemma derivers_impl_in_stack:
   sorry
 
 (* FIXME: Does not hold. *)
-lemma deriver_impl_ex_hist:
+lemma deriver_imp_ex_hist:
   assumes 
     "Prods G' \<turnstile> \<gamma>@Nt A#map Tm u \<Rightarrow>r* \<delta>@Nt B#map Tm v"
 obtains \<rho> \<sigma> where     
@@ -411,15 +411,8 @@ obtains \<rho> \<sigma> where
     "hist \<sigma> = \<delta>"
   oops
 
+*)
 
-
-
-lemma last_Nt:
-  assumes "\<alpha>@\<beta>@\<gamma>@map Tm u = \<delta>@Nt A#map Tm v"
-    "Nt A \<in> set \<beta>"
-    "Nt A \<notin> set \<gamma>"
-  obtains \<zeta> w x where "\<beta> = \<zeta> @ Nt A # map Tm w" "\<gamma> = map Tm x"
-  sorry
 
 lemma derivers_append_map_Tm:
   assumes "P \<turnstile> \<alpha> \<Rightarrow>r* u"
@@ -432,21 +425,1046 @@ lemma derivers_prepend:
   shows "P \<turnstile> \<alpha>@\<beta> \<Rightarrow>r* \<alpha> @ u"
   using assms derivern_prepend rtranclp_power by (smt (verit))+
 
+lemma syms_split_last_eq_imp_tl_eq:
+  assumes "\<alpha> @ Nt A # map Tm w = \<beta> @ Nt A # \<gamma> @ map Tm v"
+    "Nt A \<notin> set \<gamma>"
+  obtains u where "\<gamma> = map Tm u" "w = u@v"
+  using assms proof (induction w arbitrary: thesis v \<gamma> rule: rev_induct)
+  case Nil
+  from Nil(2) have A_last: "last (\<beta> @ Nt A # \<gamma> @ map Tm v) = Nt A" 
+    by (simp add: snoc_eq_iff_butlast)
+  have "\<gamma> @ map Tm v = []" 
+    by (rule ccontr)
+      (metis append.right_neutral last_ConsR last_appendR last_in_set last_map list.distinct(1)
+        list.map_disc_iff sym.distinct(1) Nil(3) A_last)
+  then show ?case using Nil by auto
+next
+  case (snoc a w)
+  from snoc(3) have butlast_eq: "\<alpha> @ Nt A # map Tm w = \<beta> @ Nt A # butlast (\<gamma> @ map Tm v)"
+  proof -
+    have "\<gamma> @ map Tm v \<noteq> []"
+      by standard (use snoc(3) in auto)
+    then obtain \<delta> b where "\<gamma> @ map Tm v = \<delta> @ [b]" using rev_exhaust by meson
+    with snoc(3) show ?thesis by force
+  qed
+  let ?\<delta> = "butlast (\<gamma> @ map Tm v)"
+  obtain \<delta> v' where \<delta>v'_def: "\<delta>@map Tm v' = ?\<delta>" by fast
+  note \<delta>v'_eq = butlast_eq[unfolded this[symmetric]]
+  from \<delta>v'_def snoc(4) have "Nt A \<notin> set \<delta>" 
+  proof -
+    from \<delta>v'_def have "set \<delta> \<subseteq> set ?\<delta>" 
+      by (metis Un_iff set_append subsetI) 
+    also have "... \<subseteq> set (\<gamma> @ map Tm v)" 
+      by (meson in_set_butlastD subsetI)
+    finally show ?thesis using snoc(4) by auto
+  qed
+  from snoc(1)[OF _ \<delta>v'_eq this] obtain u where "\<delta> = map Tm u" "w = u @ v'" by blast
+  then show thesis using snoc(2,3) \<delta>v'_def \<delta>v'_eq append_same_eq
+    by (smt (verit, ccfv_threshold) list.inject map_Tm_inject_iff map_eq_append_conv
+        same_append_eq)
+qed
 
- 
-lemma deriver_decomp:
-  assumes "P \<turnstile> [Nt A] \<Rightarrow>r* \<gamma>' @ Nt B # map Tm w"
-    "[Nt A] \<noteq> \<gamma>' @ Nt B # map Tm w"
+corollary syms_decomp_rightmost:
+  assumes "\<alpha> @ Nt A # map Tm w = \<beta> @ \<gamma> @ \<delta> @ map Tm x"
+    "Nt A \<in> set \<gamma>" "Nt A \<notin> set \<delta>"
+  obtains \<eta> u v where "\<gamma> = \<eta> @ Nt A # map Tm u" "\<delta> = map Tm v"  "w = u@v@x"
+proof -
+  from split_list_last[OF assms(2)] obtain \<zeta> \<theta> where \<gamma>_decomp: "\<gamma> = \<zeta> @ Nt A # \<theta>" "Nt A \<notin> set \<theta>" 
+    by blast
+  with assms(1) have "\<alpha> @ Nt A # map Tm w = \<beta> @ \<zeta> @ Nt A # \<theta> @ \<delta> @ map Tm x" by simp
+  moreover from \<gamma>_decomp(2) assms(3) have "Nt A \<notin> set (\<theta>@\<delta>)" by simp
+  ultimately obtain y where y_defs: "\<theta>@\<delta> = map Tm y" "w = y @ x" 
+    using syms_split_last_eq_imp_tl_eq[of \<alpha> A _ "\<beta>@\<zeta>" "\<theta>@\<delta>" _] by auto
+  then obtain u v where "\<theta> = map Tm u" "\<delta> = map Tm v" "w = u@v@x" 
+    using append_eq_map_conv y_defs by (metis append.assoc)
+  then show thesis using that \<gamma>_decomp 
+    by blast
+qed
+
+corollary syms_decomp_rightmost2:
+  assumes "\<alpha> @ Nt A # map Tm w = \<beta> @ \<gamma> @ map Tm x"
+    "Nt A \<in> set \<gamma>"
+  obtains \<delta> u where "\<gamma> = \<delta> @ Nt A # map Tm u" "w = u@x"
+proof -
+  from assms(1) have 1: "\<alpha> @ Nt A # map Tm w = \<beta> @ \<gamma> @ [] @ map Tm x" by simp
+  obtain \<delta> u v where "\<gamma> = \<delta> @ Nt A # map Tm u" "[] = map Tm v" "w = u@v@x"
+    using syms_decomp_rightmost[OF 1 assms(2) _] by auto
+  then show thesis using that by blast
+qed
+
+lemma no_Nts_imp_Tms:
+  assumes "\<nexists>A. Nt A \<in> set \<alpha>"
+  obtains w where "\<alpha> = map Tm w"
+  using assms by (metis sym.exhaust ex_map_conv)
+
+lemma syms_split_rightmost:
+  assumes "\<exists>A. Nt A \<in> set \<alpha>"
+  obtains \<beta> A u where "\<alpha> = \<beta> @ Nt A # map Tm u"
+  using assms proof (induction "length \<alpha>" arbitrary: \<alpha> thesis rule: less_induct)
+  case less
+  then obtain X \<beta> where \<alpha>_def: "\<alpha> = X#\<beta>" 
+    by (metis list.set_cases)
+  show ?case 
+  proof (cases "\<exists>A. Nt A \<in> set \<beta>")
+    case True
+    show thesis using less(1)[OF _ _ True] less(2) unfolding \<alpha>_def 
+      by (metis Cons_eq_appendI length_Cons lessI)
+  next
+    case False
+    show ?thesis using no_Nts_imp_Tms[OF False] less(2)[of "[]"] less(3) False 
+      unfolding \<alpha>_def by force
+  qed
+qed
+
+
+
+lemma deriver_cases[consumes 1, case_names rightmost Tms_only]:
+  assumes "P \<turnstile> \<alpha> \<Rightarrow>r \<beta>"
+  obtains \<gamma> A u \<gamma>' B v where "\<alpha> = \<gamma> @ Nt A # map Tm u" "\<beta> = \<gamma>' @ Nt B # map Tm v" |
+          \<gamma> A u v where "\<alpha> = \<gamma> @ Nt A # map Tm u" "\<beta> = map Tm v"
+proof -
+  from assms obtain \<gamma> A u \<delta> where \<alpha>\<beta>_defs: "\<alpha> = \<gamma> @ Nt A # map Tm u" "\<beta> = \<gamma> @ \<delta> @ map Tm u"
+    using deriver.cases by meson
+  consider "\<nexists>B. Nt B \<in> set \<delta>" | B where "Nt B \<in> set \<delta>" by blast
+  then show thesis
+  proof cases
+    case 1
+    from no_Nts_imp_Tms[OF 1] show ?thesis 
+      by (meson \<alpha>\<beta>_defs(1) syms_split_rightmost no_Nts_imp_Tms that(1,2)) 
+  next
+    case 2
+    then show ?thesis using syms_split_rightmost \<alpha>\<beta>_defs 
+      by (metis no_Nts_imp_Tms that(1,2))
+  qed
+qed
+
+
+
+
+(* induct set? *)
+lemma stepcnt_induct[consumes 1, case_names base step]:
+  assumes
+    "r\<^sup>*\<^sup>* a b"
+    "P a"
+    "\<And>n y z. \<lbrakk>(r ^^ n) a y; r y z; P y\<rbrakk> \<Longrightarrow> P z"
+  shows "P b"
+proof -
+  from assms(1) obtain n where "(r ^^ n) a b" 
+    by (metis rtranclp_power)
+  then show ?thesis 
+    by (induction n arbitrary: b) (use assms(2-) in auto)
+qed
+
+lemma stepcnt_induct2[consumes 1, case_names base step]:
+  assumes
+    "r\<^sup>*\<^sup>* a b"
+    "P a"
+    "\<And>n z. \<lbrakk>\<And>y. (r ^^ n) a y \<Longrightarrow> P y; (r ^^ Suc n) a z\<rbrakk> \<Longrightarrow> P z"
+  shows "P b"
+proof -
+  from assms(1) obtain n where "(r ^^ n) a b" 
+    by (metis rtranclp_power)
+  then show ?thesis
+    by (induction n arbitrary: b) (use assms(2-) in auto)
+qed
+
+
+
+(*
+
+lemma derive_imp_derive_Nt:
+  assumes "P \<turnstile> [Nt A] \<Rightarrow>r* \<delta>"
+    "P \<turnstile> \<delta> \<Rightarrow>r \<gamma>' @ Nt B # map Tm w"
     "P = Prods G''"
     "reduced G''"
     "LangS G'' \<noteq> {}"
+    "Eps_free P"
   obtains X \<alpha> \<alpha>' \<beta> \<beta>' v v' where
     "P \<turnstile> [Nt A] \<Rightarrow>r* \<alpha>@Nt X#\<beta>"
     "P \<turnstile> \<alpha>@Nt X#\<beta> \<Rightarrow>r* \<alpha>@Nt X#map Tm v"
     "P \<turnstile> \<alpha>@Nt X#map Tm v \<Rightarrow>r \<alpha>@\<alpha>'@Nt B#\<beta>'@map Tm v"
     "P \<turnstile> \<alpha>@\<alpha>'@Nt B#\<beta>'@map Tm v \<Rightarrow>r* \<alpha>@\<alpha>'@ Nt B#map Tm (v'@v)" 
     "\<gamma>' = \<alpha>@\<alpha>'" "w = v'@v"
-  using assms(1,2) proof (induction "\<gamma>' @ Nt B # map Tm w" arbitrary: \<gamma>' B w thesis rule: rtranclp_induct)
+
+(*proof (cases "[Nt A] = \<delta>")
+  case True
+  with assms have A_step: "P \<turnstile> [Nt A] \<Rightarrow>r \<gamma>' @ Nt B # map Tm w" by auto
+  then show ?thesis using assms that
+    by (smt (verit, ccfv_threshold) True append.assoc append.right_neutral append.right_neutral
+        deriver.cases list.map_disc_iff rtranclp.rtrancl_refl same_append_eq self_append_conv2)
+next
+  case False
+  note A_neq_\<delta> = this
+  obtain \<alpha> C x \<beta> where \<delta>_prod: "\<delta> = \<alpha> @ Nt C # map Tm x" "(C,\<beta>) \<in> P"
+    "\<alpha> @ \<beta> @ map Tm x = \<gamma>' @ Nt B # map Tm w" 
+    using deriver.cases[OF assms(2)] by metis
+  then show ?thesis 
+  proof (cases "Nt B \<in> set \<beta>")
+    case True
+    from \<delta>_prod syms_decomp_rightmost2[OF _ True] obtain \<zeta> u where "\<beta> = \<zeta> @ Nt B # map Tm u"
+      "w = u@x" by metis
+    then show ?thesis using that[of _ _ _ _ \<zeta> _] \<delta>_prod assms 
+      by (smt (verit, best) Cons_eq_appendI append_assoc append_same_eq map_append rtranclp.simps)
+  next
+    case False
+    with that \<delta>_prod show thesis
+    proof (induction "length (\<gamma>'@Nt B#map Tm w)" arbitrary: \<gamma>' \<delta> \<alpha> C x \<beta> B w thesis rule: less_induct)
+      case less
+      from less(3-) have "Nt B \<in> set \<alpha>" 
+      by (metis Nts_syms_Nil Nts_syms_append Nts_syms_map_Tm Un_iff append.right_neutral 
+          in_Nts_syms list.set_intros(1))
+    from syms_decomp_rightmost[OF _ this less(6), of _ _ "[]" x] less
+    obtain \<zeta> u v where \<alpha>_decomp: "\<alpha> = \<zeta> @ Nt B # map Tm u" "\<beta> = map Tm v" "w = u@v@x" 
+      by (metis self_append_conv2)
+    moreover from this have "length (\<zeta> @ Nt B # map Tm u) < length (\<gamma>' @ Nt B # map Tm w)" 
+    proof -
+      thm less
+      show ?thesis sorry
+    qed
+(* TODO fix this mess *)
+    ultimately obtain \<eta> X \<theta> y \<eta>' \<theta>' y' where
+      "P \<turnstile> [Nt A] \<Rightarrow>r* \<eta> @ Nt X # \<theta>" "P \<turnstile> \<eta> @ Nt X # \<theta> \<Rightarrow>r* \<eta> @ Nt X # map Tm y"
+      "P \<turnstile> \<eta> @ Nt X # map Tm y \<Rightarrow> \<eta> @ \<eta>' @ Nt B # \<theta>' @ map Tm y"
+      "P \<turnstile> \<eta> @ \<eta>' @ Nt B # \<theta>' @ map Tm y \<Rightarrow>r* \<eta> @ \<eta>' @ Nt B # map Tm (y' @ y)"
+      "\<zeta> = \<eta> @ \<eta>'" "u = y' @ y" 
+      using less(1)[of \<zeta> B u _ dd xx gg "[]" "map Tm u"] less(3) less.prems 
+      
+    with less \<alpha>_decomp show thesis 
+      using \<open>length \<zeta> < length \<gamma>'\<close> by force
+      
+
+    then show ?case using less(1)[of \<zeta> B u "\<zeta> @ [Nt B]" "map Tm u" "[]"] less(3) 
+      sorry
+    qed
+
+
+
+    with \<delta>_prod have "Nt B \<in> set \<alpha>" 
+      by (metis Nts_syms_Nil Nts_syms_append Nts_syms_map_Tm Un_iff append.right_neutral 
+          in_Nts_syms list.set_intros(1))
+    from syms_decomp_rightmost[OF _ this False, of _ _ "[]" x] \<delta>_prod(3)
+    obtain \<zeta> u v where \<alpha>_decomp: "\<alpha> = \<zeta> @ Nt B # map Tm u" "\<beta> = map Tm v" "w = u@v@x" 
+      by (metis self_append_conv2)
+    thm less(1)
+    then show ?thesis using step(4)[of \<alpha>1 X1 \<beta>1 v1 \<alpha>1' \<beta>1'] \<delta>_prod
+  qed
+qed 
+
+
+
+
+
+
+
+
+
+
+
+
+
+
+  using assms(1,2) proof (induction "length \<gamma>'" arbitrary: \<delta> \<gamma>' B w rule: less_induct)
+  case less
+  then show ?case 
+  proof (cases "[Nt A] = \<delta>")
+    case True
+    with less have A_step: "P \<turnstile> [Nt A] \<Rightarrow>r \<gamma>' @ Nt B # map Tm w" by auto
+    then show ?thesis using less
+      by (smt (verit, ccfv_threshold) True append.assoc append.right_neutral append.right_neutral
+          deriver.cases list.map_disc_iff rtranclp.rtrancl_refl same_append_eq self_append_conv2)
+  next
+    case False
+    note A_neq_\<delta> = this
+    obtain \<alpha> C x \<beta> where \<delta>_prod: "\<delta> = \<alpha> @ Nt C # map Tm x" "(C,\<beta>) \<in> P"
+      "\<alpha> @ \<beta> @ map Tm x = \<gamma>' @ Nt B # map Tm w" 
+      using deriver.cases[OF less(4)] by metis
+    then show ?thesis 
+    proof (cases "Nt B \<in> set \<beta>")
+      case True
+      from \<delta>_prod syms_decomp_rightmost2[OF _ True] obtain \<zeta> u where "\<beta> = \<zeta> @ Nt B # map Tm u"
+        "w = u@x" by metis
+      then show ?thesis using less(2)[of _ _ _ _ \<zeta> _] \<delta>_prod less(1,3-4) 
+        by (smt (verit, best) Cons_eq_appendI append_assoc append_same_eq map_append rtranclp.simps)
+    next
+      case False
+      with \<delta>_prod have "Nt B \<in> set \<alpha>" 
+        by (metis Nts_syms_Nil Nts_syms_append Nts_syms_map_Tm Un_iff append.right_neutral 
+            in_Nts_syms list.set_intros(1))
+      from syms_decomp_rightmost[OF _ this False, of _ _ "[]" x] \<delta>_prod(3)
+      obtain \<zeta> u v where \<alpha>_decomp: "\<alpha> = \<zeta> @ Nt B # map Tm u" "\<beta> = map Tm v" "w = u@v@x" 
+        by (metis self_append_conv2)
+      thm less(1)
+      then show ?thesis using step(4)[of \<alpha>1 X1 \<beta>1 v1 \<alpha>1' \<beta>1'] \<delta>_prod
+    qed
+  qed
+qed 
+
+
+
+
+
+  using assms(1,2) proof (induction arbitrary: \<gamma>' B w rule: rtranclp_induct)
+  case base
+  then show ?case
+    by (metis append.right_neutral append_Nil list.simps(8) rtranclp.rtrancl_refl)
+next
+  case (step \<delta> \<gamma>)
+  then show ?case
+  proof (cases "[Nt A] = \<delta>")
+    case True
+    with step have A_step: "P \<turnstile> [Nt A] \<Rightarrow>r \<gamma>" by auto
+    then show ?thesis
+    proof (cases rule: deriver_cases)
+      case (rightmost _ _ _  \<zeta> D v)
+      note rightmost = rightmost(2)
+      then obtain \<iota> where \<gamma>_prod: "\<zeta> @ \<iota> @ map Tm v = \<gamma>' @ Nt B # map Tm w" "(D,\<iota>) \<in> P" 
+        using deriver_imp_handle step(5) by meson
+      then show ?thesis 
+      proof (cases "Nt B \<in> set \<iota>")
+        case True
+        from syms_decomp_rightmost2[OF \<gamma>_prod(1)[symmetric] True] obtain \<theta> u where 
+          \<iota>_decomp: "\<iota> = \<theta> @ Nt B # map Tm u" "w = u @ v" by blast
+        with A_step \<iota>_decomp \<gamma>_prod(1) step(4-) rightmost show thesis by fastforce
+      next
+        case False
+        with \<gamma>_prod(1) have "Nt B \<in> set \<zeta>"
+          by (metis Nts_syms_map_Tm Un_iff empty_iff in_Nts_syms in_set_conv_decomp set_append)
+        with \<gamma>_prod(1) False syms_decomp_rightmost[OF _ this False, of _ _ "[]" v]
+        obtain \<eta> u x where "\<zeta> = \<eta> @ Nt B # map Tm u" "\<iota> = map Tm x" "w = u @ x @ v"
+          using that by auto
+        with A_step rightmost \<gamma>_prod(1) step(5)
+          step(4)[of "[]" A "[]" "[]" \<eta>] show thesis by fastforce
+      qed
+    next
+      case (Tms_only \<eta> C u v)
+      then show ?thesis using step 
+        by (metis deriver_imp_derive not_derive_map_Tm)
+    qed
+  next
+    case False
+    note A_neq_\<delta> = this
+    from step(5) obtain \<alpha> C x \<beta> where \<gamma>_prod: "\<gamma> = \<alpha> @ Nt C # map Tm x" "(C,\<beta>) \<in> P"
+      "\<alpha> @ \<beta> @ map Tm x = \<gamma>' @ Nt B # map Tm w" 
+      using deriver.cases[OF step(5)] by metis
+    then show ?thesis 
+    proof (cases "Nt B \<in> set \<beta>")
+      case True
+      from \<gamma>_prod syms_decomp_rightmost2[OF _ True] obtain \<zeta> u where "\<beta> = \<zeta> @ Nt B # map Tm u"
+        "w = u@x" by metis
+      then show ?thesis using step(4)[of _ _ _ _ \<zeta> _] \<gamma>_prod step(1-2,5) 
+        by (smt (verit, best) Cons_eq_appendI append_assoc append_same_eq map_append rtranclp.simps)
+    next
+      case False
+      with \<gamma>_prod have "Nt B \<in> set \<alpha>" 
+        by (metis Nts_syms_Nil Nts_syms_append Nts_syms_map_Tm Un_iff append.right_neutral 
+            in_Nts_syms list.set_intros(1))
+      from syms_decomp_rightmost[OF _ this False, of _ _ "[]" x] \<gamma>_prod(3)
+      obtain \<zeta> u v where \<alpha>_decomp: "\<alpha> = \<zeta> @ Nt B # map Tm u" "\<beta> = map Tm v" "w = u@v@x" 
+        by (metis self_append_conv2)
+      with \<gamma>_prod step(2,5) 
+        (* TODO: prove that if an Nt is in a string, there exists a step that produced it *)
+      then show ?thesis using step(3) \<gamma>_prod 
+    qed
+  qed
+qed
+
+
+
+
+
+
+
+    then show ?thesis sorry
+  next
+    case False
+    then show ?thesis sorry
+  qed
+qed 
+
+ using assms(1,2) proof (induction arbitrary: \<gamma>' B w thesis rule: stepcnt_induct)
+  case base
+  then show ?case 
+    by (metis append.right_neutral append_Nil list.simps(8) rtranclp.rtrancl_refl)
+next
+  case (step n \<delta> \<gamma>)
+  then show ?case proof (induction n arbitrary: \<gamma> \<delta> \<gamma>' B w  thesis rule: less_induct)
+    case (less n)
+    show ?case 
+    proof (cases n)
+      case 0
+      with less have A_step: "P \<turnstile> [Nt A] \<Rightarrow>r \<gamma>" by auto
+      then show ?thesis
+      proof (cases rule: deriver_cases)
+        case (rightmost _ _ _  \<zeta> D v)
+        note rightmost = rightmost(2)
+        then obtain \<iota> where \<gamma>_prod: "\<zeta> @ \<iota> @ map Tm v = \<gamma>' @ Nt B # map Tm w" "(D,\<iota>) \<in> P" 
+          using deriver_imp_handle less(6) by meson
+        then show ?thesis 
+        proof (cases "Nt B \<in> set \<iota>")
+          case True
+          from syms_decomp_rightmost2[OF \<gamma>_prod(1)[symmetric] True] obtain \<theta> u where 
+            \<iota>_decomp: "\<iota> = \<theta> @ Nt B # map Tm u" "w = u @ v" by blast
+          with A_step \<iota>_decomp \<gamma>_prod(1) less(5-) rightmost show thesis by fastforce
+        next
+          case False
+          with \<gamma>_prod(1) have "Nt B \<in> set \<zeta>"
+            by (metis Nts_syms_map_Tm Un_iff empty_iff in_Nts_syms in_set_conv_decomp set_append)
+          with \<gamma>_prod(1) False syms_decomp_rightmost[OF _ this False, of _ _ "[]" v]
+          obtain \<eta> u x where "\<zeta> = \<eta> @ Nt B # map Tm u" "\<iota> = map Tm x" "w = u @ x @ v"
+            using that by auto
+          with A_step rightmost \<gamma>_prod(1) less(6)
+            less(5)[of "[]" A "[]" "[]" \<eta>] show thesis by fastforce
+        qed
+      next
+        case (Tms_only \<eta> C u v)
+        then show ?thesis using less 
+          by (metis deriver_imp_derive not_derive_map_Tm)
+      qed
+    next
+      case (Suc m)
+      obtain \<alpha> C x \<beta> where \<gamma>_prod: "\<gamma> = \<alpha> @ Nt C # map Tm x" "(C,\<beta>) \<in> P"
+        "\<alpha> @ \<beta> @ map Tm x = \<gamma>' @ Nt B # map Tm w" 
+        using deriver.cases[OF less(6)] by metis
+      then show ?thesis
+      proof (cases "Nt B \<in> set \<beta>")
+        case True
+        from \<gamma>_prod syms_decomp_rightmost2[OF _ True] obtain \<zeta> u where "\<beta> = \<zeta> @ Nt B # map Tm u"
+          "w = u@x" by metis
+        then show ?thesis using less(5)[of \<alpha> C "map Tm x" x \<zeta> "map Tm u"] \<gamma>_prod less(1-4,6)
+          by (metis (no_types, lifting) ext append.assoc append_Cons append_same_eq map_append 
+              rtranclp.simps rtranclp_power) 
+      next
+        case False
+        with \<gamma>_prod have "Nt B \<in> set \<alpha>" 
+          by (metis Nts_syms_Nil Nts_syms_append Nts_syms_map_Tm Un_iff append.right_neutral 
+              in_Nts_syms list.set_intros(1))
+        from syms_decomp_rightmost[OF _ this False, of _ _ "[]" x] \<gamma>_prod(3)
+        obtain \<zeta> u v where \<alpha>_decomp: "\<alpha> = \<zeta> @ Nt B # map Tm u" "\<beta> = map Tm v" "w = u@v@x" 
+          by (metis self_append_conv2)
+        thm less(1)[of m \<eta> \<delta> C \<alpha> x]  less(4)
+        then show ?thesis sorry
+      qed
+    qed
+  qed
+qed *) *)
+
+lemma derivers_tl_substring:
+  assumes "P \<turnstile> \<alpha> @ Nt A # map Tm v \<Rightarrow>r* \<beta> @ Nt B # map Tm w"
+  obtains u where "w = u@v"
+  using assms proof (induction "\<beta> @ Nt B # map Tm w" arbitrary: \<beta> B w thesis)
+  case base
+  then show ?case using right_derivs_eq_imp_eq_tl[OF base(1)] by blast
+next
+  case (step y \<beta> B w)
+  then obtain \<gamma> C u where y_def: "y = \<gamma> @ Nt C # map Tm u" 
+    by (metis deriver_cases)
+  with step(3) obtain x where u_decomp: "u = x@v" by blast
+  from step(2) obtain \<delta> where "\<beta> @ Nt B # map Tm w = \<gamma> @ \<delta> @ map Tm u" 
+    unfolding y_def using deriver_imp_handle by metis
+  with syms_decomp_rightmost show ?case using u_decomp sorry
+qed
+
+lemma deriver_rightmost_cases[consumes 1, case_names prod prefix]:
+  assumes "P \<turnstile> \<alpha> @ Nt A # map Tm u \<Rightarrow>r \<beta> @ Nt B # map Tm w"
+  obtains \<gamma> v where "\<beta> @ Nt B # map Tm w = \<alpha> @ \<gamma> @ Nt B # map Tm v @ map Tm u" |
+          \<delta> v x where "\<alpha> = \<delta> @ Nt B # map Tm x" "\<beta> @ Nt B # map Tm w = \<alpha> @ map Tm (v@u)"
+proof -
+  from assms obtain \<gamma> where deriv: "\<beta> @ Nt B # map Tm w = \<alpha> @ \<gamma> @ map Tm u" "(A, \<gamma>) \<in> P" 
+    by (metis deriver_imp_handle)
+  then consider (Tms) x where "\<gamma> = map Tm x" | (Nt) \<delta> C \<zeta> where "\<gamma> = \<delta> @ Nt C # \<zeta>" 
+    by (metis split_list no_Nts_imp_Tms)
+  then show ?thesis 
+  proof cases
+    case Tms
+    with deriv have "\<beta> @ Nt B # map Tm w = \<alpha> @ map Tm (x@u)" by auto
+    moreover from this obtain \<delta> v where "\<alpha> = \<delta> @ Nt B # map Tm v" 
+      by (metis Nts_syms_append Nts_syms_map_Tm append.right_neutral append_Nil in_Nts_syms 
+          in_set_conv_decomp list.simps(8) syms_decomp_rightmost2)
+    ultimately show ?thesis using deriv that by blast
+  next
+    case Nt
+    obtain \<eta> D y where "Nt C # \<zeta> = \<eta> @ Nt D # map Tm y" 
+        by (meson list.set_intros(1) syms_split_rightmost)
+   moreover from this have "B = D" using deriv Nt right_derivs_eq_imp_eq_tl[of \<beta> B w "\<alpha> @ \<delta> @ \<eta>" D "y@u"]
+     by simp
+   ultimately show ?thesis using Nt that deriv by (metis append.assoc append_Cons)
+  qed
+qed
+
+
+lemma derivers_Nt_imp_last_produced:
+  assumes "P \<turnstile> [Nt A] \<Rightarrow>r(Suc n) \<gamma>"
+    "Nt B \<in> set \<gamma>"
+  obtains C \<alpha> \<beta> \<delta> v where "P \<turnstile> [Nt A] \<Rightarrow>r* \<delta> @ Nt C # map Tm v"
+    "P \<turnstile> \<delta> @ Nt C # map Tm v \<Rightarrow>r \<delta> @ \<alpha> @ Nt B # \<beta> @ map Tm v"
+    "P \<turnstile> \<delta> @ \<alpha> @ Nt B # \<beta> @ map Tm v \<Rightarrow>r* \<gamma>"
+    "Nt B \<notin> set \<beta>"
+  using assms proof (induction n arbitrary: \<gamma>)
+  case 0
+  from 0(2) show ?case using 0(1)[of "[]" A "[]"] split_list[OF 0(3)] 
+    by (metis "0.prems"(3) Nil_is_map_conv append_Nil2 in_set_conv_decomp_last relpowp_Suc_0
+        rtranclp.rtrancl_refl self_append_conv2)
+next
+  case (Suc n)
+  then obtain \<delta> where \<delta>_def: "P \<turnstile> [Nt A] \<Rightarrow>r(Suc n) \<delta>" "P \<turnstile> \<delta> \<Rightarrow>r \<gamma>" by auto
+  show ?case 
+  proof (cases "Nt B \<in> set \<delta>")
+    case True
+    then show ?thesis using Suc \<delta>_def rtranclp.rtrancl_into_rtrancl
+      by (smt (verit, best))
+  next
+    case False
+    from \<delta>_def obtain \<zeta> C v \<eta> where yz_defs: "\<delta> = \<zeta> @ Nt C # map Tm v" "\<gamma> = \<zeta> @ \<eta> @ map Tm v"
+        "(C, \<eta>) \<in> P" by (meson deriver.cases)
+      moreover with \<delta>_def(2) Suc(4) False obtain \<alpha> \<beta> where "\<eta> = \<alpha> @ Nt B # \<beta>" "Nt B \<notin> set \<beta>"
+        using split_list_last by force 
+      ultimately show ?thesis using \<delta>_def Suc
+        by (metis (no_types, lifting) append.assoc append_Cons relpowp_imp_rtranclp rtranclp.simps)
+  qed
+qed
+
+lemma derivers_imp_derivers_tl:
+  assumes "P \<turnstile> [Nt A] \<Rightarrow>r* \<alpha> @ Nt A # map Tm v"
+  obtains \<beta> where "P \<turnstile> [Nt A] \<Rightarrow>r* \<alpha> @ Nt A # \<beta>"
+    "P \<turnstile> \<alpha> @ Nt A # \<beta> \<Rightarrow>r* \<alpha> @ Nt A # map Tm v"
+  using assms by induction (use that assms in auto)
+thm deriver.cases
+inductive rm_chain :: "('a, 'b) Prods \<Rightarrow> ('a, 'b) syms \<Rightarrow> ('a, 'b) item list \<Rightarrow> ('a, 'b) syms 
+                            \<Rightarrow> bool" 
+   (\<open>_ \<Turnstile> _ \<Rightarrow>r* _ \<Rightarrow>r* _\<close> 30) for P where
+
+refl[intro]: "P \<Turnstile> \<alpha> \<Rightarrow>r* [] \<Rightarrow>r* \<alpha>" |
+
+(*step[intro]:  "\<lbrakk>P \<turnstile> \<alpha> @ Nt A # map Tm v \<Rightarrow>r \<alpha> @ \<alpha>'@ Nt B # \<beta> @ map Tm v; P \<turnstile> \<beta> \<Rightarrow>r* map Tm u\<rbrakk>
+    \<Longrightarrow> P \<Turnstile> \<alpha> @ Nt A # map Tm v \<Rightarrow>r* [[A \<rightarrow> \<alpha>' . Nt B # \<beta>]] \<Rightarrow>r* \<alpha> @ \<alpha>' @ Nt B # map Tm u @ map Tm v " | *)
+
+(* step_Tms[intro]: "P \<turnstile> \<alpha> @ Nt A # map Tm v \<Rightarrow>r \<alpha> @ map Tm u @ map Tm v 
+    \<Longrightarrow> P \<Turnstile> \<alpha> @ Nt A # map Tm v \<Rightarrow>r* [[A \<rightarrow> [] . map Tm u]] \<Rightarrow>r* \<alpha> @ map Tm u @ map Tm v" | *)
+
+step[intro]:  "\<lbrakk>P \<Turnstile> \<alpha>\<^sub>0 \<Rightarrow>r* \<rho> \<Rightarrow>r* \<alpha> @ Nt X # map Tm v; 
+    P \<turnstile> \<alpha> @ Nt X # map Tm v \<Rightarrow>r \<alpha> @ \<alpha>' @ Nt Y # \<beta> @ map Tm v; P \<turnstile> \<beta> \<Rightarrow>r* map Tm u\<rbrakk>
+    \<Longrightarrow> P \<Turnstile> \<alpha>\<^sub>0 \<Rightarrow>r* [X \<rightarrow> \<alpha>' . Nt Y # \<beta>]#\<rho> \<Rightarrow>r* \<alpha> @ \<alpha>' @ Nt Y # map Tm u @ map Tm v"
+
+
+lemma rm_chain_Tms_impossible[simp]:
+  assumes "P \<Turnstile> \<alpha> \<Rightarrow>r* [A \<rightarrow> x#xs . map Tm u]#\<rho> \<Rightarrow>r* \<beta>"
+  shows False
+  using assms by cases auto
+
+lemma rm_chain_imp_Nt_hd[elim]:
+  assumes "P \<Turnstile> \<alpha> \<Rightarrow>r* [A \<rightarrow> \<alpha>' . \<beta>]#\<rho> \<Rightarrow>r* \<gamma>"
+  obtains B \<beta>' where "\<beta> = Nt B # \<beta>'"
+  using assms by cases auto
+
+
+(* using inductive_cases adds the impossible Nil case *)
+(*
+lemma rm_chain_stepE[elim]:
+  assumes "P \<Turnstile> \<alpha> \<Rightarrow>r* [[A \<rightarrow> \<alpha>' . Nt B # \<beta>]] \<Rightarrow>r* \<gamma>"
+  obtains \<delta> v u where 
+    "\<alpha> = \<delta> @ Nt A # map Tm v" "\<gamma> = \<delta> @ \<alpha>' @ Nt B # map Tm u @ map Tm v"
+    "P \<turnstile> \<delta> @ Nt A # map Tm v \<Rightarrow>r \<delta> @ \<alpha>' @ Nt B # \<beta> @ map Tm v"
+    "P \<turnstile> \<beta> \<Rightarrow>r* map Tm u"
+  using assms by cases (use that rm_chain_impossible in fastforce)+ *)
+
+(*lemma rm_chain_step_TmsE[elim]:
+  assumes "P \<Turnstile> \<alpha> \<Rightarrow>r* [[A \<rightarrow> \<alpha>' . map Tm u]] \<Rightarrow>r* \<gamma>"
+  obtains \<delta> v where 
+    "\<alpha> = \<delta> @ Nt A # map Tm v" "\<alpha>' = []" "\<gamma> = \<delta> @ map Tm u @ map Tm v"
+    "P \<turnstile> \<delta> @ Nt A # map Tm v \<Rightarrow>r \<delta> @ map Tm u @ map Tm v"
+  using assms by cases (use that rm_chain_impossible in fastforce)+*)
+
+inductive_cases rm_chain_reflE[elim]: "P \<Turnstile> \<alpha> \<Rightarrow>r* [] \<Rightarrow>r* \<beta>"
+inductive_cases rm_chain_stepE[elim]: "P \<Turnstile> \<alpha> \<Rightarrow>r* [A \<rightarrow> \<alpha>' . Nt B # \<beta>]#\<rho> \<Rightarrow>r* \<gamma>"
+
+(*inductive_cases rm_chain_steps_TmsE[elim]: "P \<Turnstile> \<alpha> \<Rightarrow>r* [A \<rightarrow> \<alpha>' . map Tm u]#i#\<rho> \<Rightarrow>r* \<gamma>"*)
+
+lemma rm_chain_imp_prod:
+  assumes "P \<Turnstile> \<alpha>\<^sub>0 \<Rightarrow>r* [A \<rightarrow> \<alpha> . \<beta>]#\<rho> \<Rightarrow>r* \<gamma>"
+  shows "(A, \<alpha>@\<beta>) \<in> P"
+  using assms syms_split_rightmost by cases (simp add: deriver_imp_in_Prods)
+
+
+
+lemma Nt_in_chain_imp_produced:
+  assumes "P \<Turnstile> \<alpha>\<^sub>0 \<Rightarrow>r* \<rho> \<Rightarrow>r* \<gamma> @ Nt X # map Tm v"
+    "Nt B \<in> set \<gamma>"
+  obtains "is" A \<alpha> \<beta> js \<delta> u where "\<rho> = is @ [A \<rightarrow> \<alpha> . Nt B # \<beta>] # js"
+    "P \<Turnstile> \<alpha>\<^sub>0 \<Rightarrow>r* js \<Rightarrow>r* \<delta> @ Nt A # map Tm u"
+  oops
+
+
+
+lemma rm_chain_singleton_imp_eq:
+  assumes "P \<Turnstile> \<alpha>\<^sub>0 \<Rightarrow>r* [A \<rightarrow> \<alpha> . Nt C # \<beta>]#\<rho> \<Rightarrow>r* \<gamma> @ Nt B # map Tm w"
+  shows "C = B \<and> (\<exists>u v. w = u @ v \<and> P \<turnstile> \<beta> \<Rightarrow>r* map Tm u)"
+  using assms proof cases
+  case (step \<alpha>' v u)
+  with right_derivs_eq_imp_eq_tl[of _ _ _ "\<alpha>' @ \<alpha>" C] have "w = u @ v"
+    by fastforce
+  moreover with step have "C = B" by simp
+  ultimately show ?thesis using step by blast 
+qed
+
+
+
+lemma rm_chain_imp_hd_prod_rightmost:
+  assumes "P \<Turnstile> \<alpha>\<^sub>0 \<Rightarrow>r* \<rho> \<Rightarrow>r* \<gamma> @ Nt B # map Tm w"
+  obtains A \<alpha> \<beta> "is" u v where "\<rho> = [A \<rightarrow> \<alpha> . Nt B # \<beta>] # is"
+    "P \<turnstile> \<beta> \<Rightarrow>r* map Tm u" "w = u @ v" | "\<alpha>\<^sub>0 = \<gamma> @ Nt B # map Tm w"
+using assms proof cases
+  case (step \<rho> \<alpha> X v \<alpha>' Y \<beta> u)
+  moreover with right_derivs_eq_imp_eq_tl[of _ _ _ "\<alpha> @ \<alpha>'"] have "w = u@v" by simp
+  moreover from this have "B = Y" using step(2) by simp
+  ultimately show ?thesis using that by blast
+qed argo
+
+
+
+lemma rm_chain_imp_derivers:
+  assumes "P \<Turnstile> \<alpha> \<Rightarrow>r* \<rho> \<Rightarrow>r* \<beta>"
+  shows "P \<turnstile> \<alpha> \<Rightarrow>r* \<beta>"
+  using assms proof induction
+  case (step \<alpha>\<^sub>0 \<rho> \<alpha> X v \<alpha>' Y \<beta> u)
+  from step(3) derivers_append_map_Tm[OF step(3)] have
+    "P \<turnstile>  \<alpha> @ \<alpha>' @ Nt Y # \<beta> @ map Tm v \<Rightarrow>r*  \<alpha> @ \<alpha>' @ Nt Y # map Tm u @ map Tm v"
+    by (metis append_Cons append_Nil derivers_prepend)
+  then show ?case using step by simp
+qed simp
+
+lemma app_derivers_app:
+  assumes "P \<turnstile> \<alpha> \<Rightarrow>r* map Tm u"
+    "P \<turnstile> \<beta> \<Rightarrow>r* map Tm v"
+  shows "P \<turnstile> \<alpha> @ \<beta> \<Rightarrow>r* map Tm (u@v)"
+  using assms derivers_iff_derives by (metis derives_append_map_Tm)
+
+lemma syms_append_cases[consumes 1, case_names left right]:
+  assumes "\<alpha> @ Nt X # map Tm w = \<beta> @ \<gamma>"
+  obtains u v where "\<beta> = \<alpha> @ Nt X # map Tm u" "\<gamma> = map Tm v" "w = u @ v" |
+          \<delta> where "\<alpha> = \<beta> @ \<delta>" "\<delta> @ Nt X # map Tm w = \<gamma>"
+proof (cases "Nt X \<in> set \<gamma>")
+  case True
+  with syms_decomp_rightmost[of \<alpha> X w \<beta> \<gamma> "[]" "[]"]
+  show ?thesis using assms using that(2) by force
+next
+  case False
+  with assms have "Nt X \<in> set \<beta>" 
+    by (metis in_set_conv_decomp Un_iff set_append)
+  with syms_decomp_rightmost[of \<alpha> X w "[]" \<beta> \<gamma> "[]"]
+  show ?thesis using False that(1) Cons_eq_appendI assms by force
+qed
+
+thm syms_decomp_rightmost
+lemma derivers_singleton_imp_rm_chain:
+  assumes "P \<turnstile> [Nt A] \<Rightarrow>r(Suc n) \<alpha> @ Nt X # map Tm v"
+    "P = Prods J"
+    "reduced J"
+    "LangS J \<noteq> {}"
+    "A \<in> Nts P"
+  obtains \<rho> where "P \<Turnstile> [Nt A] \<Rightarrow>r* \<rho> \<Rightarrow>r* \<alpha> @ Nt X # map Tm v"
+  using assms(1) proof (induction n arbitrary: \<alpha> X v thesis)
+  case 0
+  then show ?case using rm_chain.step[of P "[Nt A]" "[]" "[]" A "[]" \<alpha> X] by auto
+next
+  case (Suc n)
+  from Suc(3) obtain \<beta> B u \<gamma> where Suc_steps: "P \<turnstile> [Nt A] \<Rightarrow>r(Suc n) \<beta> @ Nt B # map Tm u"
+    "\<beta> @ \<gamma> @ map Tm u = \<alpha> @ Nt X # map Tm v" "P \<turnstile> \<beta> @ Nt B # map Tm u \<Rightarrow>r \<beta> @ \<gamma> @ map Tm u"
+    using deriver.cases by (smt (verit, del_insts) relpowp_Suc_E)
+  from Suc(1)[OF _ this(1)] obtain \<rho> where last_chain_step: "P \<Turnstile> [Nt A] \<Rightarrow>r* \<rho> \<Rightarrow>r* \<beta> @ Nt B # map Tm u" 
+    by blast
+
+
+  from  last_chain_step Suc_steps(2,3) Suc(2) show thesis
+  proof (induction "length \<rho>" arbitrary: \<rho>  B  \<beta> u X \<gamma> \<alpha> v thesis rule: less_induct)
+    case less
+    show ?case proof (cases "Nt X \<in> set \<gamma>")
+      case True
+      from less obtain \<delta> w where"\<gamma> = \<delta> @ Nt X # map Tm w" "w @ u = v" 
+      by (metis True syms_decomp_rightmost2)
+    with less show thesis by force
+    next
+      case False
+      with less have X_in_\<beta>: "Nt X \<in> set \<beta>" 
+        by (metis Nts_syms_append Nts_syms_map_Tm Un_iff empty_iff in_Nts_syms list.set_intros(1))
+      with rm_chain_imp_hd_prod_rightmost[OF less(2)] 
+      obtain X' \<alpha>' \<beta>' "is" where 
+        \<rho>_def: "\<rho> = [X' \<rightarrow> \<alpha>' . Nt B # \<beta>'] # is" 
+        using that by cases (auto simp add: Cons_eq_append_conv)
+      from rm_chain_stepE[OF less(2)[unfolded \<rho>_def]] obtain \<zeta> w x where
+        snd_last_chn_step: 
+        "\<beta> @ Nt B # map Tm u = \<zeta> @ \<alpha>' @ Nt B # map Tm w @ map Tm x"
+        "P \<Turnstile> [Nt A] \<Rightarrow>r* is \<Rightarrow>r* \<zeta> @ Nt X' # map Tm x"
+        "P \<turnstile> \<zeta> @ Nt X' # map Tm x \<Rightarrow>r \<zeta> @ \<alpha>' @ Nt B # \<beta>' @ map Tm x"
+        "P \<turnstile> \<beta>' \<Rightarrow>r* map Tm w"
+        by metis
+      from right_derivs_eq_imp_eq_tl this(1) have uwx: "u = w @ x" 
+        by (metis append.assoc map_append)
+      with snd_last_chn_step(1) have \<beta>\<zeta>\<alpha>': "\<beta> = \<zeta> @ \<alpha>'"
+        by simp
+      from syms_decomp_rightmost[OF _ X_in_\<beta> False, of \<alpha> v "[]" u] obtain \<delta> y z where
+        \<beta>\<gamma>_decomp: "\<beta> = \<delta> @ Nt X # map Tm y" "\<gamma> = map Tm z" "v = y @ z @ u"
+        using less(3) by auto
+      have B\<beta>'_derivers: "P \<turnstile> Nt B # \<beta>' \<Rightarrow>r* map Tm z @ map Tm w" 
+      proof -
+        have "P \<turnstile> [Nt B] \<Rightarrow>r map Tm z" using deriver_singleton deriver_imp_in_Prods[OF less(4)] 
+          \<beta>\<gamma>_decomp by fast
+        from this[THEN r_into_rtranclp[of "deriver P"]] app_derivers_app snd_last_chn_step(4) 
+          show ?thesis by fastforce
+      qed
+      from \<beta>\<gamma>_decomp(3) uwx have v_decomp: "v = y @ z @ w @ x" by simp
+      note \<beta>\<gamma>_decomp(1)[unfolded \<beta>\<zeta>\<alpha>', symmetric]
+      then show thesis
+      proof (cases rule: syms_append_cases)
+        case (left u' v')
+        from \<beta>\<gamma>_decomp less(3) have \<alpha>\<delta>: "\<alpha> = \<delta>" by force
+        note \<rho>_def snd_last_chn_step(2) less(3) \<beta>\<zeta>\<alpha>' uwx
+        thm less(1)[of "is" \<zeta> X' x "\<alpha>' @ Nt B # map Tm w" \<alpha> X v]
+        thm less(1)[of js' \<alpha> X vv]
+        thm less(1)[of "is" X'' \<alpha>'' X' \<beta>'' js \<zeta> x X "\<alpha>' @ Nt B # map Tm w" \<alpha> v]
+        
+        show thesis using less(8) \<alpha>\<delta> v_decomp \<beta>\<gamma>_decomp uwx \<rho>_def sorry
+        thm rm_chain_stepE[OF snd_last_chn_step(2)[unfolded is_def]]
+        thm less(1)[of \<rho>1 X1 \<alpha>1 B1 \<beta>'1 is1] left less(2-)
+        from left snd_last_chn_step(3) have 
+          "P \<turnstile> \<delta> @ Nt X # map Tm u' @ Nt X' # map Tm x \<Rightarrow>r \<delta> @ Nt X # map Tm u' @ map Tm v'" sorry
+        show ?thesis sorry
+      next
+        case (right \<eta>)
+        with \<beta>\<gamma>_decomp less(6) have \<alpha>\<zeta>\<eta>: "\<alpha> = \<zeta>@\<eta>" by force
+        from right snd_last_chn_step(3) have 
+          "P \<turnstile> \<zeta> @ Nt X' # map Tm x \<Rightarrow>r \<zeta> @ \<eta> @ Nt X # (map Tm y @ Nt B # \<beta>') @ map Tm x"
+          by auto
+        moreover have "P \<turnstile> map Tm y @ Nt B # \<beta>' \<Rightarrow>r* map Tm (y @ z @ w)"
+          using  B\<beta>'_derivers derivers_prepend map_append by auto
+      ultimately show ?thesis using rm_chain.step[OF snd_last_chn_step(2)] less(8) \<alpha>\<zeta>\<eta>
+        v_decomp by fastforce
+      qed
+
+      then show ?thesis sorry
+    qed
+
+  qed
+
+
+
+  show ?case 
+  proof (cases "Nt X \<in> set \<gamma>")
+    case True
+    from Suc_steps(2) obtain \<delta> w where"\<gamma> = \<delta> @ Nt X # map Tm w" "w @ u = v" 
+      by (metis True syms_decomp_rightmost2)
+    with Suc Suc_steps last_chain_step show thesis by force
+  next
+    case False
+    with Suc_steps(2) have X_in_\<beta>: "Nt X \<in> set \<beta>" 
+      by (metis Nts_syms_append Nts_syms_map_Tm Un_iff empty_iff in_Nts_syms list.set_intros(1))
+    with rm_chain_imp_hd_prod_rightmost[OF last_chain_step] 
+    obtain X' \<alpha>' \<beta>' "is" where 
+      \<rho>_def: "\<rho> = [X' \<rightarrow> \<alpha>' . Nt B # \<beta>'] # is" 
+      using that by cases (auto simp add: Cons_eq_append_conv)
+
+    from this last_chain_step False X_in_\<beta> Suc_steps(2,3) Suc(2) show thesis
+    proof (induction "length \<rho>" arbitrary: \<alpha>' \<rho> X' B \<beta>' "is" \<beta> u X \<gamma> \<alpha> v thesis rule: less_induct)
+      case less
+
+      note \<rho>_def = less(2)
+      note last_chain_step = less(3)
+      note False = less(4)
+      note X_in_\<beta> = less(5)
+      from rm_chain_stepE[OF last_chain_step[unfolded \<rho>_def]] obtain \<zeta> w x where
+        snd_last_chn_step: 
+        "\<beta> @ Nt B # map Tm u = \<zeta> @ \<alpha>' @ Nt B # map Tm w @ map Tm x"
+        "P \<Turnstile> [Nt A] \<Rightarrow>r* is \<Rightarrow>r* \<zeta> @ Nt X' # map Tm x"
+        "P \<turnstile> \<zeta> @ Nt X' # map Tm x \<Rightarrow>r \<zeta> @ \<alpha>' @ Nt B # \<beta>' @ map Tm x"
+        "P \<turnstile> \<beta>' \<Rightarrow>r* map Tm w"
+        by metis
+      from right_derivs_eq_imp_eq_tl this(1) have uwx: "u = w @ x" 
+        by (metis append.assoc map_append)
+      with snd_last_chn_step(1) have \<beta>\<zeta>\<alpha>': "\<beta> = \<zeta> @ \<alpha>'"
+        by simp
+      from syms_decomp_rightmost[OF _ X_in_\<beta> False, of \<alpha> v "[]" u] obtain \<delta> y z where
+        \<beta>\<gamma>_decomp: "\<beta> = \<delta> @ Nt X # map Tm y" "\<gamma> = map Tm z" "v = y @ z @ u"
+        using less(6) by auto
+      have B\<beta>'_derivers: "P \<turnstile> Nt B # \<beta>' \<Rightarrow>r* map Tm z @ map Tm w" 
+      proof -
+        have "P \<turnstile> [Nt B] \<Rightarrow>r map Tm z" using deriver_singleton deriver_imp_in_Prods[OF less(7)] 
+          \<beta>\<gamma>_decomp by fast
+        from this[THEN r_into_rtranclp[of "deriver P"]] app_derivers_app snd_last_chn_step(4) show ?thesis
+          by fastforce
+      qed
+      from \<beta>\<gamma>_decomp(3) uwx have v_decomp: "v = y @ z @ w @ x" by simp
+      note \<beta>\<gamma>_decomp(1)[unfolded \<beta>\<zeta>\<alpha>', symmetric]
+      then show thesis
+      proof (cases rule: syms_append_cases)
+        case (left u' v')
+        from \<beta>\<gamma>_decomp less(6) have \<alpha>\<delta>: "\<alpha> = \<delta>" by force
+        from rm_chain_imp_hd_prod_rightmost[OF snd_last_chn_step(2)] 
+        obtain X'' \<alpha>'' \<beta>'' js where is_def:
+          "is = [X'' \<rightarrow> \<alpha>'' . Nt X' # \<beta>''] # js"
+          using left by cases simp+
+        moreover have "P \<Turnstile> [Nt A] \<Rightarrow>r* is \<Rightarrow>r* \<zeta> @ Nt X' # map Tm v" sorry
+        moreover from left have "Nt X \<in> set \<zeta>" "Nt X \<notin> set \<alpha>'"
+          by auto
+        thm less(1)[of "is" X'' \<alpha>'' X' \<beta>'' js \<zeta> x X "\<alpha>' @ Nt B # map Tm w" \<alpha> v]
+        
+        show thesis using less(8) \<alpha>\<delta> v_decomp \<beta>\<gamma>_decomp uwx \<rho>_def sorry
+        thm rm_chain_stepE[OF snd_last_chn_step(2)[unfolded is_def]]
+        thm less(1)[of \<rho>1 X1 \<alpha>1 B1 \<beta>'1 is1] left less(2-)
+        from left snd_last_chn_step(3) have 
+          "P \<turnstile> \<delta> @ Nt X # map Tm u' @ Nt X' # map Tm x \<Rightarrow>r \<delta> @ Nt X # map Tm u' @ map Tm v'" sorry
+        show ?thesis sorry
+      next
+        case (right \<eta>)
+        with \<beta>\<gamma>_decomp less(6) have \<alpha>\<zeta>\<eta>: "\<alpha> = \<zeta>@\<eta>" by force
+        from right snd_last_chn_step(3) have 
+          "P \<turnstile> \<zeta> @ Nt X' # map Tm x \<Rightarrow>r \<zeta> @ \<eta> @ Nt X # (map Tm y @ Nt B # \<beta>') @ map Tm x"
+          by auto
+        moreover have "P \<turnstile> map Tm y @ Nt B # \<beta>' \<Rightarrow>r* map Tm (y @ z @ w)"
+          using  B\<beta>'_derivers derivers_prepend map_append by auto
+      ultimately show ?thesis using rm_chain.step[OF snd_last_chn_step(2)] less(8) \<alpha>\<zeta>\<eta>
+        v_decomp by fastforce
+      qed
+
+
+
+      then show ?case sorry
+    qed
+
+
+
+    from rm_chain_stepE[OF last_chain_step[unfolded \<rho>_def(1)]] obtain \<zeta> w x where
+      snd_last_chn_step: 
+      "\<beta> @ Nt B # map Tm u = \<zeta> @ \<alpha>' @ Nt B # map Tm w @ map Tm x"
+      "P \<Turnstile> [Nt A] \<Rightarrow>r* is \<Rightarrow>r* \<zeta> @ Nt X' # map Tm x"
+      "P \<turnstile> \<zeta> @ Nt X' # map Tm x \<Rightarrow>r \<zeta> @ \<alpha>' @ Nt B # \<beta>' @ map Tm x"
+      "P \<turnstile> \<beta>' \<Rightarrow>r* map Tm w"
+      by metis
+    from right_derivs_eq_imp_eq_tl this(1) have uwx: "u = w @ x" 
+      by (metis append.assoc map_append)
+    with snd_last_chn_step(1) have \<beta>\<zeta>\<alpha>': "\<beta> = \<zeta> @ \<alpha>'"
+      by simp
+    from syms_decomp_rightmost[OF _ X_in_\<beta> False, of \<alpha> v "[]" u] obtain \<delta> y z where
+      \<beta>\<gamma>_decomp: "\<beta> = \<delta> @ Nt X # map Tm y" "\<gamma> = map Tm z" "v = y @ z @ u"
+      using Suc_steps(2) by auto
+
+    have B\<beta>'_derivers: "P \<turnstile> Nt B # \<beta>' \<Rightarrow>r* map Tm z @ map Tm w" 
+    proof -
+      have "P \<turnstile> [Nt B] \<Rightarrow>r map Tm z" using deriver_singleton deriver_imp_in_Prods[OF Suc_steps(3)] 
+        \<beta>\<gamma>_decomp by fast
+      from this[THEN r_into_rtranclp[of "deriver P"]] app_derivers_app snd_last_chn_step(4) show ?thesis
+        by fastforce
+    qed
+    from \<beta>\<gamma>_decomp(3) uwx have v_decomp: "v = y @ z @ w @ x" by simp
+
+    note \<beta>\<gamma>_decomp(1)[unfolded \<beta>\<zeta>\<alpha>', symmetric]
+    then show thesis
+    proof (cases rule: syms_append_cases)
+      case (left u' v')
+      from \<beta>\<gamma>_decomp Suc_steps(2) have "\<alpha> = \<delta>" by force
+      from rm_chain_imp_hd_prod_rightmost[OF snd_last_chn_step(2)] 
+      obtain X'' \<alpha>'' \<beta>'' js where is_def:
+        "is = [X'' \<rightarrow> \<alpha>'' . Nt X' # \<beta>''] # js"
+        using left by cases simp+
+      thm rm_chain_stepE[OF snd_last_chn_step(2)[unfolded is_def]]
+      from left snd_last_chn_step(3) have 
+        "P \<turnstile> \<delta> @ Nt X # map Tm u' @ Nt X' # map Tm x \<Rightarrow>r \<delta> @ Nt X # map Tm u' @ map Tm v'"
+        thm left rm_chain.step[of P "[Nt A]" "is" \<delta> X vv] Suc(2)
+      then show ?thesis sorry
+    next
+      case (right \<eta>)
+      with \<beta>\<gamma>_decomp Suc_steps(2) have \<alpha>\<zeta>\<eta>: "\<alpha> = \<zeta>@\<eta>" by force
+      from right snd_last_chn_step(3) have 
+        "P \<turnstile> \<zeta> @ Nt X' # map Tm x \<Rightarrow>r \<zeta> @ \<eta> @ Nt X # (map Tm y @ Nt B # \<beta>') @ map Tm x"
+        by auto
+      moreover have "P \<turnstile> map Tm y @ Nt B # \<beta>' \<Rightarrow>r* map Tm (y @ z @ w)"
+        using  B\<beta>'_derivers derivers_prepend map_append by auto
+    ultimately show ?thesis using rm_chain.step[OF snd_last_chn_step(2)] Suc(2) \<alpha>\<zeta>\<eta>
+      v_decomp by fastforce
+    qed
+      
+
+
+    from snd_last_chn_step(3) have 
+      "P \<turnstile> \<zeta> @ Nt X' # map Tm x \<Rightarrow>r \<delta> @ Nt X # (map Tm y @ Nt B # \<beta>') @ map Tm x"
+      using \<beta>\<zeta>\<alpha>' \<beta>\<gamma>_decomp(1) append.assoc by (metis append_Cons)
+    moreover have "P \<turnstile> map Tm y @ Nt B # \<beta>' \<Rightarrow>r* map Tm (y @ z @ w)"
+      using derivers_prepend[OF B\<beta>'_derivers] map_append by simp
+
+    (* prove that B derives tms. Prove that those tms @ u = v ( Use syms_decomp_rightmost )
+       Go one step back (the step that produces B), and "sneak" everything to the right of X into \<beta>. 
+       Then derive replace [X' \<rightarrow> \<alpha>' . Nt B # \<beta>'] with [X' \<rightarrow> \<alpha>'' . Nt X # as @ Nt B # \<beta>']
+       on top of is. as must be Tms and B derives tms, and \<alpha>' = \<alpha>'' @ Nt X # as. 
+      
+
+*)
+
+    then show ?thesis sorry
+  qed
+qed
+  
+
+ (* lemma derivers_decomp_gen:
+  assumes "P \<turnstile> [Nt A] \<Rightarrow>r(Suc n) \<gamma> @ Nt B # \<delta>"
+  obtains X \<alpha> \<alpha>' \<beta> \<beta>' v where
+    "P \<turnstile> [Nt A] \<Rightarrow>r* \<alpha>@Nt X#\<beta>"
+    "P \<turnstile> \<alpha>@Nt X#\<beta> \<Rightarrow>r* \<alpha>@Nt X#map Tm v"
+    "P \<turnstile> \<alpha>@Nt X#map Tm v \<Rightarrow>r \<alpha>@\<alpha>'@Nt B#\<beta>'@map Tm v"
+    "\<gamma> = \<alpha>@\<alpha>'" "\<delta> = \<beta>' @ map Tm v"
+  using assms proof (induction "length \<gamma>" arbitrary: \<gamma> B \<delta> thesis rule: less_induct)
+  case less
+  from derivers_Nt_imp_last_produced obtain C \<alpha> \<beta> \<gamma>' v where 
+    "P \<turnstile> [Nt A] \<Rightarrow>r* \<gamma>' @ Nt C # map Tm v"
+    "P \<turnstile> \<gamma>' @ Nt C # map Tm v \<Rightarrow>r \<gamma>' @ \<alpha> @ Nt B # \<beta> @ map Tm v"
+    "P \<turnstile> \<gamma>' @ \<alpha> @ Nt B # \<beta> @ map Tm v \<Rightarrow>r* \<gamma> @ Nt B # \<delta>" 
+    "Nt B \<notin> set \<beta>"
+    using less(3) 
+  then show ?case oops
+
+
+lemma derivers_decomp:
+  assumes "P \<turnstile> [Nt A] \<Rightarrow>r(Suc n) \<gamma>' @ Nt B # map Tm w"
+    "P = Prods G''"
+    "reduced G''"
+    "LangS G'' \<noteq> {}"
+  obtains X \<alpha> \<alpha>' \<beta> v v' where
+    "P \<turnstile> [Nt A] \<Rightarrow>r* \<alpha>@Nt X#map Tm v"
+    "P \<turnstile> \<alpha>@Nt X#map Tm v \<Rightarrow>r \<alpha>@\<alpha>'@Nt B#\<beta>@map Tm v"
+    "P \<turnstile> \<alpha>@\<alpha>'@Nt B#\<beta>@map Tm v \<Rightarrow>r* \<alpha>@\<alpha>'@ Nt B#map Tm (v'@v)" 
+    "\<gamma>' = \<alpha>@\<alpha>'" "w = v'@v"
+proof -
+  from derivers_Nt_imp_last_produced obtain C \<alpha> \<beta> \<delta> v where B_prod:
+    "P \<turnstile> [Nt A] \<Rightarrow>r* \<delta> @ Nt C # map Tm v"
+    "P \<turnstile> \<delta> @ Nt C # map Tm v \<Rightarrow>r \<delta> @ \<alpha> @ Nt B # \<beta> @ map Tm v"
+    "P \<turnstile> \<delta> @ \<alpha> @ Nt B # \<beta> @ map Tm v \<Rightarrow>r* \<gamma>' @ Nt B # map Tm w" 
+    "Nt B \<notin> set \<beta>" using assms(1,2) by (smt (verit, ccfv_SIG) in_set_conv_decomp)
+  from B_prod(3,1,2,4) that assms(1,2) show ?thesis
+  proof (induction  "\<delta> @ \<alpha> @ Nt B # \<beta> @ map Tm v" arbitrary: thesis \<delta> \<alpha> \<beta> v C rule: converse_rtranclp_induct)
+    case base
+    from base(1,4) have "\<gamma>' = \<delta>@\<alpha>" "map Tm w = \<beta> @ map Tm v"
+    proof -
+      from base(4) have "Nt B \<notin> set \<beta> \<union> set (map Tm v)" "Nt B \<notin> set (map Tm w)"
+        using sym.exhaust by auto
+      with x_notin_tl_imp_eq base(1) show "\<gamma>' = \<delta>@\<alpha>" "map Tm w = \<beta> @ map Tm v" 
+        by (metis append.assoc set_append)+
+    qed
+    then show ?case using base(5)[of \<delta> C "map Tm v" v \<alpha> \<beta>] base(1-4)
+sorry
+  next
+    case (step z)
+    then obtain \<zeta> D u where z_def: "z = \<zeta> @ Nt D # map Tm u" using deriver.cases 
+      by (metis converse_rtranclpE)
+    from step(1)[unfolded z_def] show thesis sorry
+  qed
+qed
+
+
+
+
+
+
+
+
+
+
+
+
+
+    case base
+    from base(1,4) have "\<gamma>' = \<delta>@\<alpha>" "map Tm w = \<beta> @ map Tm v"
+    proof -
+      from base(4) have "Nt B \<notin> set \<beta> \<union> set (map Tm v)" "Nt B \<notin> set (map Tm w)"
+        using sym.exhaust by auto
+      with x_notin_tl_imp_eq base(1) show "\<gamma>' = \<delta>@\<alpha>" "map Tm w = \<beta> @ map Tm v" 
+        by (metis append.assoc set_append)+
+    qed
+    then show ?case using base(5)[of \<delta> C "map Tm v" v \<alpha> \<beta>] base(1-4)
+      by (metis rtranclp.simps syms_split_last_eq_imp_tl_eq)
+  next
+    case (step y)
+    from step(2) consider
+      \<eta> u where "y = \<eta> @ Nt B # map Tm u" |
+      \<eta> C u
+    then show ?case sorry
+  qed
+qed
+    
+
+
+
+  using assms(1,2) proof (induction "length \<gamma>'" arbitrary: \<gamma>' B w thesis rule: less_induct)
+
+
+
+
+
+  using assms(1,2) proof (induction "\<gamma>' @ Nt B # map Tm w" arbitrary: \<gamma>' B w thesis)
+  case (step \<delta>)
+  obtain \<alpha> C x \<beta> where \<delta>_prod: "\<delta> = \<alpha> @ Nt C # map Tm x" "(C,\<beta>) \<in> P"
+    "\<alpha> @ \<beta> @ map Tm x = \<gamma>' @ Nt B # map Tm w" 
+    using deriver.cases[OF step(2)] by metis
+  then show ?case 
+  proof (cases "Nt B \<in> set \<beta>")
+    case True
+    from \<delta>_prod syms_decomp_rightmost2[OF _ True] obtain \<zeta> u where "\<beta> = \<zeta> @ Nt B # map Tm u"
+      "w = u@x" by metis
+    then show ?thesis using step(4)[of \<alpha> C "map Tm x" x \<zeta> "map Tm u"] \<delta>_prod step(1-3,5)
+      by (smt (verit) append.assoc append_Cons append_eq_append_conv length_Cons length_append 
+          length_map relpowp_imp_rtranclp rtranclp.rtrancl_refl)
+  next
+    case False
+    with \<delta>_prod have "Nt B \<in> set \<alpha>" 
+      by (metis Nts_syms_Nil Nts_syms_append Nts_syms_map_Tm Un_iff append.right_neutral 
+          in_Nts_syms list.set_intros(1))
+    from syms_decomp_rightmost[OF _ this False, of _ _ "[]" x] \<delta>_prod(3)
+    obtain \<zeta> u v where \<alpha>_decomp: "\<alpha> = \<zeta> @ Nt B # map Tm u" "\<beta> = map Tm v" "w = u@v@x" 
+      by (metis self_append_conv2)
+    hence \<delta>B_def: "\<delta> = \<zeta> @ Nt B # map Tm u @ Nt C # map Tm x" using \<delta>_prod by simp
+    from derivers_Nt_imp_produced[OF step(1) _ this] obtain X \<alpha>' \<beta>' \<eta> y where
+      "P \<turnstile> [Nt A] \<Rightarrow>r* \<eta> @ Nt X # map Tm y" "P \<turnstile> \<eta> @ Nt X # map Tm y \<Rightarrow>r \<eta> @ \<alpha>' @ Nt B # \<beta>' @ map Tm y"
+      "P \<turnstile> \<eta> @ \<alpha>' @ Nt B # \<beta>' @ map Tm y \<Rightarrow>r* \<delta>" by (metis Un_iff \<delta>_prod(1) \<open>Nt B \<in> set \<alpha>\<close> set_append)
+    then show ?thesis sorry
+
+
+
+
+  then show ?case proof (induction n arbitrary: \<delta> \<gamma>' B w rule: less_induct)
+    case (less n)
+    then show ?case
+    proof (cases n)
+      case 0
+      with less have "P \<turnstile> [Nt A] \<Rightarrow>r \<gamma>' @ Nt B # map Tm w" by simp
+      then show ?thesis using less(5)[of "[]" A "[]" "[]"] by auto
+    next
+      case (Suc m)
+      obtain \<alpha> C x \<beta> where \<delta>_prod: "\<delta> = \<alpha> @ Nt C # map Tm x" "(C,\<beta>) \<in> P"
+        "\<alpha> @ \<beta> @ map Tm x = \<gamma>' @ Nt B # map Tm w" 
+        using deriver.cases[OF less(3)] by metis
+      then show ?thesis 
+      proof (cases "Nt B \<in> set \<beta>")
+        case True
+        from \<delta>_prod syms_decomp_rightmost2[OF _ True] obtain \<zeta> u where "\<beta> = \<zeta> @ Nt B # map Tm u"
+          "w = u@x" by metis
+        then show ?thesis using less(5)[of \<alpha> C "map Tm x" x \<zeta> "map Tm u"] \<delta>_prod less(1-4,6)
+          by (metis (no_types, lifting) ext append.assoc append_Cons append_same_eq map_append 
+              rtranclp.simps rtranclp_power) 
+      next
+        case False
+        with \<delta>_prod have "Nt B \<in> set \<alpha>" 
+          by (metis Nts_syms_Nil Nts_syms_append Nts_syms_map_Tm Un_iff append.right_neutral 
+              in_Nts_syms list.set_intros(1))
+        from syms_decomp_rightmost[OF _ this False, of _ _ "[]" x] \<delta>_prod(3)
+        obtain \<zeta> u v where \<alpha>_decomp: "\<alpha> = \<zeta> @ Nt B # map Tm u" "\<beta> = map Tm v" "w = u@v@x" 
+          by (metis self_append_conv2)
+        hence \<delta>B_def: "\<delta> = \<zeta> @ Nt B # map Tm u @ Nt C # map Tm x" using \<delta>_prod by simp
+        with derivers_Nt_imp_produced[OF step]
+        then show ?thesis sorry
+      qed
+    qed
+  qed
+qed satx
+
+
+  using assms(1,2) proof (induction "\<gamma>' @ Nt B # map Tm w" arbitrary: \<gamma>' B w thesis 
+                          rule: rtranclp_induct)
   case (step \<delta>)
   show ?case
   proof (cases "[Nt A] = \<delta>", goal_cases single_step steps)
@@ -455,47 +1473,31 @@ lemma deriver_decomp:
       by (metis append.right_neutral append_Nil list.simps(8) rtranclp.rtrancl_refl)
   next
     case steps
-    from step(2) obtain C \<zeta> u \<eta> where \<delta>_prod: "\<delta> = \<zeta> @ Nt C # map Tm u" "(C, \<eta>) \<in> P" 
+    moreover from step(2) obtain C \<zeta> u \<eta> where \<delta>_prod: "\<delta> = \<zeta> @ Nt C # map Tm u" "(C, \<eta>) \<in> P" 
       "\<zeta>@\<eta>@map Tm u = \<gamma>'@Nt B # map Tm w"
       using deriver.cases by metis
-    from step(3)[OF \<delta>_prod(1) _ steps[unfolded this(1)]] obtain \<alpha> X \<beta> v \<alpha>' \<beta>' v' where \<delta>_decomp:
-      "P \<turnstile> [Nt A] \<Rightarrow>r* \<alpha>@Nt X#\<beta>" "P \<turnstile> \<alpha>@Nt X#\<beta> \<Rightarrow>r* \<alpha>@Nt X#map Tm v" 
-      "P \<turnstile> \<alpha>@Nt X#map Tm v \<Rightarrow>r \<alpha>@\<alpha>'@Nt C#\<beta>'@map Tm v" 
-      "P \<turnstile> \<alpha>@\<alpha>'@Nt C#\<beta>'@map Tm v \<Rightarrow>r* \<alpha>@\<alpha>'@Nt C#map Tm (v'@v)" 
-      "\<zeta> = \<alpha>@\<alpha>'" "u = v'@v" using assms(3-) by blast
-    note aux = step(4)[of \<zeta> C "\<beta>'@map Tm v" "v'@v"] 
-
-
-    from  \<delta>_prod(3) consider "Nt B \<in> set \<eta>" | "Nt B \<in> set \<zeta> \<and> Nt B \<notin> set \<eta>"
-      by (metis Nts_syms_Nil Nts_syms_append Nts_syms_map_Tm Un_iff append.right_neutral in_Nts_syms
-          list.set_intros(1))
-    then show ?case proof cases
-      case 1
-      then obtain \<theta> \<iota> where \<eta>_decomp: "\<theta> @ Nt B # \<iota> = \<eta>" "Nt B \<notin> set \<iota>"
-        by (metis split_list_last)
-      with \<delta>_prod have \<iota>_is_Tms: "\<iota> @ map Tm u = map Tm w"
-        sorry
-      moreover then obtain x where \<iota>_def: "\<iota> = map Tm x" 
-        by (metis append_eq_map_conv)
-      moreover from \<delta>_decomp have "P \<turnstile> [Nt A] \<Rightarrow>r* \<zeta> @ Nt C # \<beta>' @ map Tm v" 
-         "P \<turnstile> \<zeta> @ Nt C # \<beta>' @ map Tm v \<Rightarrow>r* \<zeta> @ Nt C # map Tm (v' @ v)"
-         "P \<turnstile> \<zeta> @ Nt C # map Tm (v' @ v) \<Rightarrow>r \<zeta> @ \<theta> @ Nt B # \<iota> @ map Tm (v' @ v)"
-         "P \<turnstile> \<zeta> @ \<theta> @ Nt B # \<iota> @ map Tm (v' @ v) \<Rightarrow>r* \<zeta> @ \<theta> @ Nt B # map Tm (x @ v' @ v)"
-          apply simp
-        using \<delta>_decomp apply simp
-        using \<delta>_prod \<eta>_decomp deriver.cases 
-         \<delta>_decomp(6) step.hyps(2) apply force
-        using \<iota>_def by simp
-      moreover have "\<gamma>' = \<zeta> @ \<theta>" using \<delta>_prod(3) \<eta>_decomp \<iota>_is_Tms 
-        by fastforce
-      ultimately show ?thesis using \<delta>_decomp 
-        by (metis (mono_tags, lifting) map_Tm_inject_iff map_append step.prems(1)) 
-    next
-      case 2
-      then show ?thesis sorry
-    qed
+    ultimately show thesis using derive_imp_derive_Nt[OF step(1,2)] step(3,4) steps 
+      by (metis assms(3-))
   qed
 qed simp
+
+lemma rtranclp_step_imp_Suc:
+  assumes "P \<turnstile> \<alpha> \<Rightarrow>r* \<beta>"
+    "P \<turnstile> \<beta> \<Rightarrow>r \<gamma>"
+  obtains n where "P \<turnstile> \<alpha> \<Rightarrow>r(Suc n) \<gamma>"
+  using rtranclp_imp_relpowp[OF assms(1)] assms(2) by auto
+
+
+lemma converse_rtranclp_step_imp_Suc:
+  assumes "P \<turnstile> \<alpha> \<Rightarrow>r \<beta>"
+    "P \<turnstile> \<beta> \<Rightarrow>r* \<gamma>"
+  obtains n where "P \<turnstile> \<alpha> \<Rightarrow>r(Suc n) \<gamma>"
+proof -
+  from assms(1) have "P \<turnstile> \<alpha> \<Rightarrow>r(Suc 0) \<beta>" by auto
+  also from rtranclp_imp_relpowp[OF assms(2)] obtain n where "P \<turnstile> \<beta> \<Rightarrow>r(n) \<gamma>" by blast
+  finally show thesis using that by simp
+qed
+
 
 
     (* New approach: we show that A must be in the stack, reachable by X as seen above. 
@@ -506,25 +1508,46 @@ qed simp
       Previous approach: induct over n steps. Problem: last step does not produce A in general
       Possibly: induct over n steps with weak induction obtaining X and m where
         S' \<Rightarrow>r(m) \<gamma>Xu \<Rightarrow>r \<gamma>\<delta>A\<zeta>u \<Rightarrow>r* \<gamma>'Aw with m < n *)
-lemma deriver_impl_IPDA_comp:
+*)
+lemma deriver_imp_IPDA_comp:
   assumes "Prods G' \<turnstile> [Nt S'] \<Rightarrow>r* \<gamma>'@Nt A#map Tm w"
     "Prods G' \<turnstile> \<gamma>'@Nt A#map Tm w \<Rightarrow>r \<gamma>'@\<alpha>@\<beta>@map Tm w"
     "Prods G' \<turnstile> \<beta> \<Rightarrow>r* map Tm v"
   obtains \<rho> where 
     "([A \<rightarrow> \<alpha> . \<beta>]#\<rho>@[init_symbol IPDA], v@w) \<turnstile>P* ([I.final_state, init_symbol IPDA], [])" 
     "hist \<rho> = \<gamma>'"
+  sorry
+
+
+
+(*
   using assms(1) proof cases
   case rtrancl_refl
   then have step: "\<gamma>' = [] \<and> w = [] \<and> \<alpha>@\<beta> = [Nt S]"
-    using assms(2) S'_derive_impl_S append_eq_Cons_conv deriver_imp_derive by fastforce
+    using assms(2) S'_derive_imp_S append_eq_Cons_conv deriver_imp_derive by fastforce
   then show ?thesis 
     by (metis I.hist_init I.init_symbol_ipda append.right_neutral append_Nil assms(3)
-        derivers_S_append_impl_comp hist_singleton local.rtrancl_refl map_Tm_Nt_eq_map_Tm_Nt that)
+        derivers_S_append_imp_comp hist_singleton local.rtrancl_refl map_Tm_Nt_eq_map_Tm_Nt that)
 next
   case (rtrancl_into_rtrancl b)
-  then show ?thesis sorry
+  then obtain n where "Prods G' \<turnstile> [Nt S'] \<Rightarrow>r(Suc n) \<gamma>' @ Nt A # map Tm w"
+    using rtranclp_step_imp_Suc by blast
+  from derivers_decomp[OF this _ G'_reduced G'_not_empty] obtain X \<alpha>' \<gamma> \<beta>' u v' where decomp:
+    "Prods G' \<turnstile> [Nt S'] \<Rightarrow>r* \<gamma> @ Nt X # map Tm v'" 
+    "Prods G' \<turnstile> \<gamma> @ Nt X # map Tm v' \<Rightarrow>r \<gamma> @ \<alpha>' @ Nt A # \<beta>' @ map Tm v'"
+    "Prods G' \<turnstile> \<gamma> @ \<alpha>' @ Nt A # \<beta>' @ map Tm v' \<Rightarrow>r* \<gamma> @ \<alpha>' @ Nt A # map Tm (u@v')"
+    "u@v' = w" "\<gamma> @ \<alpha>' = \<gamma>'" by metis
+  then obtain \<rho> "is" where "\<rho> = [X \<rightarrow> \<alpha>' . Nt A # \<beta>'] # is" by blast  
+  with decomp show ?thesis 
+  proof (induction "is" arbitrary: X \<alpha>' A \<beta>')
+    case Nil
+    then show ?case sorry
+  next
+    case (Cons a "is")
+    then show ?case sorry
+  qed
 qed
-qed
+
 
 
 
@@ -535,30 +1558,30 @@ qed
   case base
   then have "\<gamma>' = [] \<and> w = []" "\<alpha>@\<beta> = [Nt S]"
     by (simp add: Cons_eq_append_conv,
-        metis (no_types, opaque_lifting) S'_derive_impl_S append_Nil2 derive_singleton 
+        metis (no_types, opaque_lifting) S'_derive_imp_S append_Nil2 derive_singleton 
         deriver_singleton list.exhaust list.simps(3) Cons_eq_append_conv)
   then show ?case using base unfolding hist_defs
-    by (metis append.left_neutral append.right_neutral concat.simps(1) derivers_S_append_impl_comp 
+    by (metis append.left_neutral append.right_neutral concat.simps(1) derivers_S_append_imp_comp 
         list.inject list.simps(8) sym.inject(1))
 next
   case (step \<gamma>)
   then obtain as where \<alpha>_derivers: "Prods G' \<turnstile> \<alpha> \<Rightarrow>r* map Tm as"
-    using reduced_derived_substring_impl_derives[OF _ G'_reduced G'_not_empty] G'_def 
+    using reduced_derived_substring_imp_derives[OF _ G'_reduced G'_not_empty] G'_def 
     by (metis (no_types, lifting) Cfg.sel(2) derivers_iff_derives derivers_imp_derives
         rtranclp.rtrancl_into_rtrancl)
   obtain X \<delta> u where \<gamma>_def: "\<gamma> = \<delta> @ Nt X#map Tm u"
     using step(2) by (meson deriver.cases)
   then obtain xs ys where xy_defs: "(X, xs@ys) \<in> Prods G'" "\<delta>@xs@ys@map Tm u = \<gamma>'@Nt A#map Tm w"
-    using step deriver_impl_handle by (metis self_append_conv2)
+    using step deriver_imp_handle by (metis self_append_conv2)
   with step obtain v' where ys_derivers: "Prods G' \<turnstile> ys \<Rightarrow>r* map Tm v'"
-    using reduced_derived_substring_impl_derives[OF _ G'_reduced G'_not_empty] G'_def \<gamma>_def 
+    using reduced_derived_substring_imp_derives[OF _ G'_reduced G'_not_empty] G'_def \<gamma>_def 
     by (metis (no_types, lifting) Cfg.sel(2) append.assoc derivers_iff_derives derivers_imp_derives
         rtranclp.rtrancl_into_rtrancl)
-  with step(2,3) obtain \<rho> where \<rho>_def:
+  with step(2,3) obtain \<rho> where last_chain_step:
     "([X \<rightarrow> xs . ys]#\<rho>@[init_symbol IPDA], v'@u) \<turnstile>P* ([final_state, init_symbol IPDA],[])"
     "hist \<rho> = \<delta>"
     using \<gamma>_def xy_defs by metis
-  with reaches_final_impl_compl_final have X_compl_final:
+  with reaches_final_imp_compl_final have X_compl_final:
     "([X \<rightarrow> xs@ys . []]#\<rho>@[init_symbol IPDA], u) \<turnstile>P* ([final_state, init_symbol IPDA],[])"
     using ys_derivers derivers_imp_derives sorry
   obtain Y ws zs \<rho>l \<rho>r where Y_defs:
@@ -570,16 +1593,16 @@ next
       "Prods G' \<turnstile> \<delta> @ Nt X # map Tm u \<Rightarrow>r \<delta> @ (xs @ ys) @ map Tm u" by auto
      have 3: "Prods G' \<turnstile> \<alpha>@\<beta> \<Rightarrow>r* map Tm (as @ v)"
        using \<alpha>_derivers step(6) by (meson derivers_iff_derives derives_append_map_Tm)
-     show thesis using that derivers_impl_in_stack[OF _ 2 _ _ 3 X_compl_final] xy_defs(2) 
+     show thesis using that derivers_imp_in_stack[OF _ 2 _ _ 3 X_compl_final] xy_defs(2) 
        by (metis (no_types, lifting) \<gamma>_def append.assoc append.simps(2) step.hyps(1) step.prems(2))
    qed
    let ?\<rho>' = "[Y \<rightarrow> ws . Nt A#zs]#\<rho>r"
   note Y_defs(2)
   also have Y_step: 
     "(?\<rho>'@[init_symbol IPDA], as@v@w) \<turnstile>P ([A \<rightarrow> [] . \<alpha>@\<beta>]#?\<rho>'@[init_symbol IPDA], as@v@w)"
-    using expanding deriver_impl_in_Prods step(5) 
+    using expanding deriver_imp_in_Prods step(5) 
     by (metis (no_types, lifting) append.assoc append_Cons)
-  also with derivers_impl_completes have A_init_steps:
+  also with derivers_imp_completes have A_init_steps:
     "... \<turnstile>P* ([A \<rightarrow> \<alpha> . \<beta>]#?\<rho>'@[init_symbol IPDA], v@w)"
     using \<alpha>_derivers by (metis append_Nil rtranclp_power)
   finally have ex_comp: "... \<turnstile>P* ([final_state, init_symbol IPDA], [])"
@@ -587,11 +1610,11 @@ next
   moreover have "hist ?\<rho>' = \<gamma>'" 
   proof -
     from Y_defs(2) Y_step A_init_steps 
-    derivers_impl_completes rtranclp_imp_relpowp step(6)
+    derivers_imp_completes rtranclp_imp_relpowp step(6)
     have "([X \<rightarrow> xs @ ys . []]#\<rho>@[init_symbol IPDA], u) \<turnstile>P* ([A \<rightarrow> \<alpha>@\<beta> . []]#?\<rho>'@[init_symbol IPDA],w)"
       using rtranclp_trans 
       by (smt (verit, ccfv_threshold) append.right_neutral rtranclp.rtrancl_into_rtrancl)
-    with \<gamma>_def step(2) xy_defs(2) X_compl_final show ?thesis using \<rho>_def(2) sorry
+    with \<gamma>_def step(2) xy_defs(2) X_compl_final show ?thesis using last_chain_step(2) sorry
   qed
   ultimately show ?case using step(4) by presburger
 qed
@@ -599,29 +1622,29 @@ qed
 
 
 
-(*
+
     (* Does not hold in general. Strong induction needed instead *)
     obtain \<delta>' u' where X_prod: "(X, \<delta>'@Nt A#map Tm u') \<in> Prods G'" "\<gamma>' = \<delta>@\<delta>'" 
       "map Tm (u'@u) = map Tm w"
       using deriver_decomp[OF n_steps(2)] by blast
-    from reduced_derived_substring_impl_derives[OF _ G'_reduced G'_not_empty] 
+    from reduced_derived_substring_imp_derives[OF _ G'_reduced G'_not_empty] 
     Suc.prems(4) obtain v' where A_derives: "Prods G' \<turnstile> [Nt A] \<Rightarrow>r* map Tm v'"
      by (metis (no_types, opaque_lifting) append_Cons append_self_conv2
         derivern_imp_deriven derivers_iff_derives rtranclp_power)
     hence A_Cons_derivers: "Prods G' \<turnstile> Nt A#map Tm u' \<Rightarrow>r* map Tm (v'@u')" 
       using derives_append derivers_iff_derives by (metis append_Cons append_Nil map_append)
-    from Suc(1)[OF _ this _ n_steps(1)] obtain \<rho> where \<rho>_def:
+    from Suc(1)[OF _ this _ n_steps(1)] obtain \<rho> where last_chain_step:
       "([X \<rightarrow> \<delta>' . Nt A#map Tm u'] # \<rho> @ [init_symbol IPDA], v' @ u' @ u) \<turnstile>P* (?qf, [])"
       "hist \<rho> = \<delta>"
       using n_steps(2) X_prod(2,3) append_assoc by (metis append_Cons map_Tm_inject_iff map_append)
     hence Xw_final: "([X \<rightarrow> \<delta>' @ [Nt A] . map Tm u'] # \<rho> @ [init_symbol IPDA], w) \<turnstile>P* (?qf, [])"
-      using derives_impl_complete_reaches_final Suc(3) derivers_iff_derives 
+      using derives_imp_complete_reaches_final Suc(3) derivers_iff_derives 
       by (metis A_derives X_prod(3) append_Cons append_Nil map_Tm_inject_iff) 
     let ?\<rho>' = "[X \<rightarrow> \<delta>' . Nt A#map Tm u'] # \<rho>"
-    have \<rho>'_hist: "hist ?\<rho>' = \<gamma>'" using \<rho>_def(2) X_prod(2) by (simp add: history_def)
+    have \<rho>'_hist: "hist ?\<rho>' = \<gamma>'" using last_chain_step(2) X_prod(2) by (simp add: history_def)
     have "([A \<rightarrow> \<alpha> . \<beta>] # ?\<rho>' @ [init_symbol IPDA], v@w) 
       \<turnstile>P* ([A \<rightarrow> \<alpha>@\<beta> . []]# ?\<rho>' @ [init_symbol IPDA], w)" 
-      using derives_impl_completes derivers_iff_derives Suc(3) 
+      using derives_imp_completes derivers_iff_derives Suc(3) 
       by (metis append.right_neutral)
     also have "... \<turnstile>P ([X \<rightarrow> \<delta>' @ [Nt A] . map Tm u'] # \<rho> @ [init_symbol IPDA], w)"
       using LR_Parser.IPDA.reducing[OF ipda] by simp
