Escallon/LR_Parsing/Extended_Cfg.thy
@@ -4,8 +4,8 @@ theory Extended_Cfg
 begin
 
 
-(* A generic list lemma *)
-lemma index_gt_left_impl_right:
+(* generic list lemmas *)
+lemma index_gt_left_imp_right:
   assumes "length xs < m" "m < length (xs@y#ys)"
         shows "(xs@y#ys)!m \<in> set ys"
 proof -
@@ -18,8 +18,32 @@ proof -
         length_append less_Suc_eq not_less_eq nth_mem zero_less_diff)
 qed
 
+lemma x_notin_tl_imp_eq:
+  assumes "ws @ x # xs = ys @ x # zs"
+  "x \<notin> set xs" "x \<notin> set zs"
+shows "ws = ys \<and> xs = zs"
+  using assms proof (induction xs arbitrary: zs rule: rev_induct)
+  case Nil
+  have "zs = []"
+    by (rule ccontr) (metis last.simps last_append last_in_set list.discI Nil(1,3))
+  then show ?case using Nil(1) by blast
+next
+  case (snoc a xs)
+  obtain a' zs' where zs_snoc: "zs = zs' @ [a']"
+  proof -
+    have "\<exists>a zs'. zs = zs' @ [a]"
+      by (rule ccontr)
+        (metis Un_insert_right last_ConsR last_appendR last_snoc list.set_intros(1) list.simps(15)
+          rev_exhaust set_append snoc(2-))
+    thus thesis using that by blast
+  qed
+  with snoc have "ws = ys \<and> xs = zs'" by force
+  then show ?case using zs_snoc snoc by blast
+qed
 
-(* Generic right derivation lemmas *)
+
+
+(* Generic derivation lemmas *)
 lemma right_derivs_eq_impossible:
   assumes "\<beta> @ Nt A # map Tm u = \<beta>' @ Nt A' # map Tm u'" (is "?w = ?w'")
     "length \<beta> < length \<beta>'" (is "?n < ?m")
@@ -27,11 +51,11 @@ lemma right_derivs_eq_impossible:
 proof -
   have inds: "?w!?n = Nt A" "?w'!?m = Nt A'" by auto 
   with assms obtain a where "?w!?m = Tm a"
-    using index_gt_left_impl_right[of \<beta> ?m "Nt A" "map Tm u", OF assms(2)] by auto
+    using index_gt_left_imp_right[of \<beta> ?m "Nt A" "map Tm u", OF assms(2)] by auto
   then show False using inds(2) assms(1) by simp
 qed
 
-lemma right_derivs_eq_impl_eq_tl:
+lemma right_derivs_eq_imp_eq_tl:
   assumes "\<beta> @ Nt A # map Tm u = \<beta>' @ Nt A' # map Tm u'"
   shows "u = u'"
 proof (rule ccontr)
@@ -47,14 +71,14 @@ proof (rule ccontr)
   qed (use assms neq in auto)
 qed
 
-lemma deriver_impl_in_Prods:
-  assumes "Prods G' \<turnstile> \<gamma> @ Nt A#map Tm w \<Rightarrow>r \<gamma>@\<alpha>@map Tm w"
-  shows "(A, \<alpha>) \<in> Prods G'"
+lemma deriver_imp_in_Prods:
+  assumes "P \<turnstile> \<gamma> @ Nt A#map Tm w \<Rightarrow>r \<gamma>@\<alpha>@map Tm w"
+  shows "(A, \<alpha>) \<in> P"
   using deriver.cases[OF assms]
-  by (metis append_eq_append_conv length_Cons list.inject right_derivs_eq_impl_eq_tl
+  by (metis append_eq_append_conv length_Cons list.inject right_derivs_eq_imp_eq_tl
       sym.inject(1))
 
-lemma deriver_impl_handle:
+lemma deriver_imp_handle:
   assumes "P \<turnstile> \<beta> @ Nt A#map Tm u \<Rightarrow>r \<gamma> @ Nt X#map Tm v"
   obtains \<alpha> where "\<beta>@\<alpha>@map Tm u = \<gamma> @ Nt X#map Tm v"
     "(A, \<alpha>) \<in> P" 
@@ -63,7 +87,20 @@ proof -
     "\<beta> @ Nt A # map Tm u = \<beta>' @ Nt A' # map Tm u'"
     "\<gamma> @ Nt X # map Tm v = \<beta>' @ \<alpha>' @ map Tm u'"
     "(A', \<alpha>') \<in> P" by metis
-  with right_derivs_eq_impl_eq_tl[OF this(1)] show thesis using that by simp
+  with right_derivs_eq_imp_eq_tl[OF this(1)] show thesis using that by simp
+qed
+
+lemma derives_Nts_subset_preserved:
+  assumes "P \<turnstile> \<alpha> \<Rightarrow>* \<beta>"
+    "Nts_syms \<alpha> \<subseteq> Nts P"
+  shows "Nts_syms \<beta> \<subseteq> Nts P"
+  using assms proof induction
+  case base
+  then show ?case .
+next
+  case (step y z)
+  from step(3)[OF step(4)] step(2) show ?case 
+    by (smt (verit, ccfv_threshold) Nts_Lhss_Rhs_Nts Un_iff derive_Nts_syms_subset subset_eq)
 qed
 
 
@@ -72,6 +109,10 @@ section \<open>Context-Free Items\<close>
 datatype ('n, 't) item = Item 'n  "('n, 't) syms"  "('n, 't) syms"
 
 notation Item  ("[_ \<rightarrow> _ . _]" 100) 
+
+
+definition prod_of_item :: "('n, 't) item \<Rightarrow> ('n, 't) prod" where
+  "prod_of_item i \<equiv> case i of [A \<rightarrow> \<alpha> . \<beta>] \<Rightarrow> (A, \<alpha>@\<beta>)"
 
 definition history :: "('n, 't) item \<Rightarrow> ('n, 't) syms" where
   "history i \<equiv> case i of [A \<rightarrow> \<alpha> . \<beta>] \<Rightarrow> \<alpha>"
@@ -191,13 +232,13 @@ A definition with variant 2, using [S' \<rightarrow> [] . []] as a dummy startin
 definition reduced :: "('n,'t) Cfg \<Rightarrow> bool" where
   "reduced G \<equiv> \<forall>A \<in> Nts (Prods G). useful (Prods G) (Start G) A"
 
-lemma Lang_nempty_impl_useful_S:
+lemma Lang_nempty_imp_useful_S:
   assumes "LangS G \<noteq> {}"
   shows "useful (Prods G) (Start G) (Start G)"
   using assms unfolding useful_def Lang_def by fastforce
 
 (* TODO mv *)
-lemma reduced_impl_restrict_useful_id: 
+lemma reduced_imp_restrict_useful_id: 
   assumes "reduced G" 
   shows  "restrict_Nts (useful (Prods G) (Start G)) (Prods G) = Prods G" (is "?R = ?P")
 proof 
@@ -207,19 +248,19 @@ proof
     unfolding restrict_Nts_def using assms Nts_def reduced_def by fastforce
 qed
 
-lemma restrict_useful_id_impl_reduced:
+lemma restrict_useful_id_imp_reduced:
   assumes "restrict_Nts (useful (Prods G) (Start G)) (Prods G) = Prods G" 
   shows "reduced G"
   using assms unfolding restrict_Nts_def reduced_def Nts_def by fast
 
-lemma reduced_impl_derives_singleton:
+lemma reduced_imp_derives_singleton:
   assumes "reduced G"
     "A \<in> Nts (Prods G)"
   obtains v where "Prods G \<turnstile> [Nt A] \<Rightarrow>* map Tm v"
   using assms productive_if_useful unfolding reduced_def 
   by metis
 
-lemma reduced_impl_derives:
+lemma reduced_imp_derives:
   assumes  "Nts_syms \<alpha> \<subseteq> Nts (Prods G)"
     "reduced G"
     "LangS G \<noteq> {}"
@@ -231,7 +272,7 @@ lemma reduced_impl_derives:
   proof (cases a)
     case (Nt A)
     with \<open>reduced G\<close> obtain u where A_derives: "Prods G \<turnstile> [Nt A] \<Rightarrow>* map Tm u"
-      using reduced_impl_derives_singleton[OF assms(2)] Cons(3) by auto
+      using reduced_imp_derives_singleton[OF assms(2)] Cons(3) by auto
     from derives_append[OF this] have "Prods G \<turnstile> Nt A#as \<Rightarrow>* map Tm u @ as" 
       by simp
     also from derives_prepend[OF as_derives] have "Prods G \<turnstile> ... \<Rightarrow>* map Tm (u@v)" 
@@ -244,7 +285,7 @@ lemma reduced_impl_derives:
   qed
 qed simp
 
-lemma derived_impl_in_Prods:
+lemma derived_imp_in_Prods:
   assumes "Start G \<in> Nts (Prods G)"
   shows "Prods G \<turnstile> [Nt (Start G)] \<Rightarrow>*\<alpha> \<Longrightarrow> Nts_syms \<alpha> \<subseteq> Nts (Prods G)"
 proof (induction rule: rtranclp_induct)
@@ -259,30 +300,30 @@ next
 qed
 
 
-corollary reduced_derived_impl_derives:
+corollary reduced_derived_imp_derives:
   assumes  "Prods G \<turnstile> [Nt (Start G)] \<Rightarrow>* \<alpha>"
     "reduced G"
     "LangS G \<noteq> {}"
   obtains v where "Prods G \<turnstile> \<alpha> \<Rightarrow>* map Tm v"
 proof - 
-  from Lang_nempty_impl_useful_S[OF assms(3)] have "Start G \<in> Nts (Prods G)"
+  from Lang_nempty_imp_useful_S[OF assms(3)] have "Start G \<in> Nts (Prods G)"
     unfolding useful_def 
     by (metis Lang_empty_if_notin_Lhss Nts_Lhss_Rhs_Nts Un_iff assms(3))
-  from derived_impl_in_Prods[OF this assms(1)] show thesis 
-    using assms(2,3) reduced_impl_derives that by blast
+  from derived_imp_in_Prods[OF this assms(1)] show thesis 
+    using assms(2,3) reduced_imp_derives that by blast
 qed
 
-corollary reduced_derived_substring_impl_derives:
+corollary reduced_derived_substring_imp_derives:
   assumes  "Prods G \<turnstile> [Nt (Start G)] \<Rightarrow>* u@\<alpha>@v"
     "reduced G"
     "LangS G \<noteq> {}"
   obtains w where "Prods G \<turnstile> \<alpha> \<Rightarrow>* map Tm w"
 proof -
-  from Lang_nempty_impl_useful_S[OF assms(3)] have "Start G \<in> Nts (Prods G)"
+  from Lang_nempty_imp_useful_S[OF assms(3)] have "Start G \<in> Nts (Prods G)"
     unfolding useful_def 
     by (metis Lang_empty_if_notin_Lhss Nts_Lhss_Rhs_Nts Un_iff assms(3))
-  from derived_impl_in_Prods[OF this assms(1)] have "Nts_syms \<alpha> \<subseteq> Nts (Prods G)" by simp
-  from reduced_impl_derives[OF this assms(2,3)] show thesis using that by blast
+  from derived_imp_in_Prods[OF this assms(1)] have "Nts_syms \<alpha> \<subseteq> Nts (Prods G)" by simp
+  from reduced_imp_derives[OF this assms(2,3)] show thesis using that by blast
 qed
 
 
@@ -317,7 +358,7 @@ lemma G'_derive_S:
   "Prods G' \<turnstile> [Nt S'] \<Rightarrow> [Nt S]"
   unfolding G'_def using derive_singleton by auto
 
-lemma G_derives_impl_G'_derives:
+lemma G_derives_imp_G'_derives:
   assumes "Prods G \<turnstile> \<alpha> \<Rightarrow>* w"
   shows "Prods G' \<turnstile> \<alpha> \<Rightarrow>* w"
   using assms G_Prods_subset_G' by (simp add: derives_mono)
@@ -332,7 +373,7 @@ corollary S'_Prod_notin_G [simp]:
   "(S', \<alpha>) \<notin> Prods G"
   using S'_notin_Nts_Prods_G unfolding Nts_def Nts_syms_def by blast
 
-lemma S'_derive_impl_S:
+lemma S'_derive_imp_S:
   assumes "Prods G' \<turnstile> [Nt S'] \<Rightarrow> \<alpha>"
   shows "\<alpha> = [Nt S]"
 proof -
@@ -348,28 +389,28 @@ proof -
   thus ?thesis by simp
 qed
 
-lemma G_derives_from_S_impl_G'_derives_from_S':
+lemma G_derives_from_S_imp_G'_derives_from_S':
   assumes "Prods G \<turnstile> [Nt S] \<Rightarrow>* w"
   shows "Prods G' \<turnstile> [Nt S'] \<Rightarrow>* w"
-  using assms G_derives_impl_G'_derives G'_derive_S
+  using assms G_derives_imp_G'_derives G'_derive_S
   by fastforce
 
-lemma G'_derives_from_S_impl_derives_from_S':
+lemma G'_derives_from_S_imp_derives_from_S':
   assumes "Prods G' \<turnstile> [Nt S] \<Rightarrow>* \<alpha>"
   shows "Prods G' \<turnstile> [Nt S'] \<Rightarrow>* \<alpha>"
   using assms G'_derive_S by simp
 
-corollary G'_derives_from_S_impl_in_Lang:
+corollary G'_derives_from_S_imp_in_Lang:
   assumes "Prods G' \<turnstile> [Nt S] \<Rightarrow>* map Tm w"
   shows "w \<in> LangS G'"
-  using G'_derives_from_S_impl_derives_from_S'[OF assms]
+  using G'_derives_from_S_imp_derives_from_S'[OF assms]
   unfolding Lang_def G'_def by simp
 
-lemma G'_derive_impl_G_derive_if_no_S':
+lemma G'_derive_imp_G_derive_if_no_S':
   "\<lbrakk>Prods G' \<turnstile> \<alpha> \<Rightarrow> \<gamma>; Nt S' \<notin> set \<alpha>\<rbrakk> \<Longrightarrow> Prods G \<turnstile> \<alpha> \<Rightarrow> \<gamma>"
   using G'_def by (simp add: derive_iff in_set_conv_decomp)
 
-lemma G'_derives_impl_G_derives_if_no_S':
+lemma G'_derives_imp_G_derives_if_no_S':
   "\<lbrakk>Prods G' \<turnstile> \<alpha> \<Rightarrow>* \<gamma>; Nt S' \<notin> set \<alpha>\<rbrakk> \<Longrightarrow> Prods G \<turnstile> \<alpha> \<Rightarrow>* \<gamma>"
 proof (induction rule: rtranclp_induct)
   case (step \<beta> \<gamma>)
@@ -377,7 +418,7 @@ proof (induction rule: rtranclp_induct)
   moreover from this have "Nt S' \<notin> set \<beta>" 
     using S'_notin_Nts_Prods_G derives_set_subset in_Nts_iff_in_Syms step.prems 
     by fastforce
-  ultimately  show ?case using step G'_derive_impl_G_derive_if_no_S'[OF step(2)]
+  ultimately  show ?case using step G'_derive_imp_G_derive_if_no_S'[OF step(2)]
     by simp
 qed simp
 
@@ -394,11 +435,11 @@ proof
     hence "Prods G' \<turnstile> [Nt S'] \<Rightarrow>* map Tm w" unfolding Lang_def G'_def by simp
     then obtain \<alpha> where "Prods G' \<turnstile> [Nt S'] \<Rightarrow> \<alpha>" "Prods G' \<turnstile> \<alpha> \<Rightarrow>* map Tm w" 
       by (meson derive_singleton derives_Nt_map_TmD)
-    from S'_derive_impl_S[OF this(1)] this(2) show "w \<in> LangS G" 
-      using G'_derives_impl_G_derives_if_no_S' S_neq_S' unfolding Lang_def by simp
+    from S'_derive_imp_S[OF this(1)] this(2) show "w \<in> LangS G" 
+      using G'_derives_imp_G_derives_if_no_S' S_neq_S' unfolding Lang_def by simp
   qed
 next
-  show "LangS G \<subseteq> LangS G'" using G_derives_from_S_impl_G'_derives_from_S'
+  show "LangS G \<subseteq> LangS G'" using G_derives_from_S_imp_G'_derives_from_S'
     unfolding Lang_def G'_def by auto
 qed
 
@@ -414,11 +455,11 @@ lemma G'_reduced:
    "reduced G'"
 proof - 
   have "\<forall>A \<in> Nts (Prods G) \<union> {S}. useful (Prods G') S' A"
-    using G_reduced G_not_empty Lang_preserved G_derives_impl_G'_derives Lang_nempty_impl_useful_S
+    using G_reduced G_not_empty Lang_preserved G_derives_imp_G'_derives Lang_nempty_imp_useful_S
     unfolding reduced_def useful_def Lang_def 
-    by (metis G_derives_from_S_impl_G'_derives_from_S' S_def Un_iff singleton_iff) 
+    by (metis G_derives_from_S_imp_G'_derives_from_S' S_def Un_iff singleton_iff) 
   moreover have "useful (Prods G') S' S'" 
-    using Lang_nempty_impl_useful_S G_not_empty Lang_preserved G'_def by fastforce
+    using Lang_nempty_imp_useful_S G_not_empty Lang_preserved G'_def by fastforce
   ultimately have "\<forall>A \<in> Nts (Prods G'). useful (Prods G') S' A"
     using Nts_G'_is_union by blast
   moreover from Nts_G'_is_union have "Nts (Prods G') = Nts (Prods G') \<union> {S'}" by blast
